($R\lor_2, L\lor$)
\begin{prooftree}
	\noLine
	\AXC{$\mathbf{D_0}'$}
	\UIC{$\Gamma \Rightarrow C$}
	\RightLabel{$R\lor_2$}
	\UIC{$\Gamma \Rightarrow B \lor C$}
	
	\noLine
	\AXC{$\Sigma , (\nabla^l (B \lor C))^{n-1} , \nabla^l B \Rightarrow \Delta$}
	\AXC{$\mathbf{D_1}'$}
	\UIC{$\Sigma , (\nabla^l (B \lor C))^{n-1} , \nabla^l C \Rightarrow \Delta$}
	\RightLabel{$L\lor$}
	\BIC{$\Sigma , (\nabla^l (B \lor C))^n \Rightarrow \Delta$}
	
	\RightLabel{$MC$} \dashedLine
	\BIC{$\nabla^l \Gamma , \Sigma \Rightarrow \Delta$}
\end{prooftree}
Induction hypothesis for $\mathbf{D_0}$ and $\mathbf{D_1}'$ gives us $\nabla^l \Gamma , \Sigma , \nabla^l C \Rightarrow \Delta$. Then we remove $C$ by a low rank $MC$ on this sequent and $\mathbf{D_0}'$ to get $\nabla^l \Gamma^2 , \Sigma \Rightarrow \Delta$, which yields the desired sequent after enough applications of $Lc$.
\begin{prooftree}
	\noLine
	\AXC{$\mathbf{D_0}'$}
	\UIC{$\Gamma \Rightarrow C$}
	
	\noLine
	\AXC{$\mathbf{D_0}$}
	\UIC{$\Gamma \Rightarrow B \lor C$}
	
	\noLine
	\AXC{$\mathbf{D_1}'$}
	\UIC{$\Sigma , (\nabla^l (B \lor C))^{n-1} , \nabla^l C \Rightarrow \Delta$}
	
	\RightLabel{IH}
	\BIC{$\nabla^l \Gamma , \Sigma , \nabla^l C \Rightarrow \Delta$}
	
	\RightLabel{$MC$}
	\BIC{$\nabla^l \Gamma^2 , \Sigma \Rightarrow \Delta$}
	
	\doubleLine \RightLabel{$Lc$}
	\UIC{$\nabla^l \Gamma , \Sigma \Rightarrow \Delta$}
\end{prooftree}