($R \nabla, Ex$) This forces $A = \bot$. So $R*$ is $R \nabla$ and $k > 0$.
		\begin{prooftree}
			\noLine
			\AXC{$\mathbf{D_0}'$}
			\UIC{$\mathcal{S} \Rightarrow \nabla^{k'} \bot$}
			\RightLabel{$R\nabla$}
			\UIC{$\p \mathcal{S} \Rightarrow \nabla^{k' + 1} \bot$}
			

			\AXC{$\mathbf{D_1}$}
			\RightLabel{$Ex$}
			\UIC{$\p^{l+k'+1} \bot^n \Rightarrow$}
			
			\dashedLine\RightLabel{$\nabla Cut$}
			\BIC{$\p^{l+1} \mathcal{S} \Rightarrow$}
		\end{prooftree}
		The desired sequent is exactly what we get from induction hypothesis for $\mathbf{D_0}'$ and $\mathbf{D_1}$.
		\begin{prooftree}
			\noLine
			\AXC{$\mathbf{D_0}'$}
			\UIC{$\mathcal{S} \Rightarrow \nabla^{k'} \bot$}
			
			\AXC{$\mathbf{D_1}$}
			\RightLabel{$Ex$}
			\UIC{$\p^{l+k'+1} \bot^n \Rightarrow$}
			
			\RightLabel{IH}
			\BIC{$\p^{l+k'+1} \mathcal{S} \Rightarrow$}
		\end{prooftree}