($R\land, L\land_1$)
		\begin{prooftree}
			\noLine
			\AXC{$\mathbf{D_0}'$}
			\UIC{$\Gamma \Rightarrow B$}
			\AXC{$\Gamma \Rightarrow C$}
			\RightLabel{$R\land$}
			\BIC{$\Gamma \Rightarrow B \land C$}
			
			\noLine
			\AXC{$\mathbf{D_1}'$}
			\UIC{$\Sigma , (\nabla^l (B \land C))^{n-1}, \nabla^l B \Rightarrow \Delta$}
			\RightLabel{$L\land_1$}
			\UIC{$\Sigma , (\nabla^l (B \land C))^n \Rightarrow \Delta$}
			
			\RightLabel{$MC$} \dashedLine
			\BIC{$\nabla^l \Gamma , \Sigma \Rightarrow \Delta$}
		\end{prooftree}
		Induction hypothesis for $\mathbf{D_0}$ and $\mathbf{D_1}'$ gives us $\nabla^l \Gamma , \Sigma , \nabla^l B \Rightarrow \Delta$. Then we remove $B$ by a low rank $MC$ on this sequent and $\mathbf{D_0}'$ to get $\nabla^l \Gamma^2 , \Sigma \Rightarrow \Delta$, which yields the desired sequent after enough applications of $Lc$.
		\begin{prooftree}
			\noLine
			\AXC{$\mathbf{D_0}'$}
			\UIC{$\Gamma \Rightarrow B$}

			\noLine
			\AXC{$\mathbf{D_0}$}
			\UIC{$\Gamma \Rightarrow B \land C$}
			\noLine
			\AXC{$\mathbf{D_1}'$}
			\UIC{$\Sigma , (\nabla^l (B \land C))^{n-1}, \nabla^l B \Rightarrow \Delta$}
			
			\RightLabel{IH}
			\BIC{$\nabla^l \Gamma , \Sigma , \nabla^l B \Rightarrow \Delta$}

			\RightLabel{$MC$}
			\BIC{$\nabla^l \Gamma^2 , \Sigma \Rightarrow \Delta$}
			
			\doubleLine \RightLabel{$Lc$}
			\UIC{$\nabla^l \Gamma , \Sigma \Rightarrow \Delta$}
		\end{prooftree}