\documentclass[a4paper, 12pt]{paper}
\usepackage{amsmath}
\usepackage{amssymb}
\usepackage{titlesec}
\usepackage{fullpage}
\usepackage{tikz-cd}
\usepackage{multicol}
\usepackage[left=.5in,right=.5in,top=.5in,bottom=.5in]{geometry}
\usepackage{enumitem}
\usepackage{bussproofs}

\setitemize{topsep=3pt,parsep=5pt,partopsep=0pt,label=,leftmargin=1.3pc}
\titleformat{\section}[runin]{\normalfont\bfseries}{\thesection}{0.5em}{}
\titlespacing{\section}{0pc}{1.5ex plus .1ex minus .2ex}{1pc}
\titleformat{\subsection}[runin]{\normalfont\bfseries}{\thesubsection}{0.7em}{}
\titlespacing{\subsection}{0pc}{2ex plus .1ex minus .2ex}{1pc}
\titleformat{\subsubsection}[runin]{\normalfont\bfseries}{\thesubsubsection}{0.7em}{}
\titlespacing{\subsubsection}{0pc}{2ex plus .1ex minus .2ex}{1pc}
\newcommand\eqn{\refstepcounter{equation}\tag{\theequation}}
\binoppenalty=\maxdimen
\relpenalty=\maxdimen
\newcommand{\ul}{\ulcorner}
\newcommand{\ur}{\urcorner}
\newcommand{\val}[1]{\ulcorner \#1 \urcorner}
\EnableBpAbbreviations

\begin{document}
{\noindent
	v 0.2 \\
{\large\textbf{The Cut Rule Is Admissible in GSTL}}
}
\\
\setcounter{section}{-1}

\input{GSTL}

\section{Theorem}\label{cut-admis} For any $\mathcal{S}$, $n$, $A$, $\mathcal{T}$, $k$, $l$ and $\Delta$, if $\text{GSTL}^-\vdash \mathcal{S} \Rightarrow \nabla^k A$ and $\text{GSTL}^-\vdash \mathcal{T} \cup [A^n | \epsilon_{k+l}] \Rightarrow \Delta$ with proof trees of ranks less than $\rho(A)$, then
 $\text{GSTL}^-\vdash [ \mathcal{S} | \epsilon_l ] \cup \mathcal{T} \Rightarrow \Delta$ also with a proof tree of a rank less than $\rho(A)$.
 
\emph{Proof:}
Let $\mathbf{D_0}$ and $\mathbf{D_1}$ be proof trees of ranks less than $\rho(A)$, with conclusions $\mathcal{S} \Rightarrow \nabla^k A$ and $\mathcal{T} \cup [A^n | \epsilon_{k+l}] \Rightarrow \Delta$ and heights $h(\mathbf{D_0})$ and $h(\mathbf{D_1})$ respectively.
\begin{prooftree}
	\noLine
	\AXC{$\mathbf{D_0}$}
	\UIC{$\mathcal{S} \Rightarrow \nabla^k A$}
	
	\noLine
	\AXC{$\mathbf{D_1}$}
	\UIC{$\mathcal{T} \cup [A^n | \epsilon_{k+l}] \Rightarrow \Delta$}
	
	\dashedLine \RightLabel{$Cut$}
	\BIC{$[ \mathcal{S} | \epsilon_l ] \cup \mathcal{T} \Rightarrow \Delta$}
\end{prooftree}
By induction on $h(\mathbf{D_0}) + h(\mathbf{D_1})$ and $\rho(A)$, the induction hypothesis states that for any proof trees $\mathbf{D_0}'$ with conclusion $\mathcal{S}' \Rightarrow \nabla^{k'} A'$ and $\mathbf{D_1}'$ with conclusion $\mathcal{T}' \cup [A'^m | \epsilon_{k'+l'}] \Rightarrow \Delta'$ such that either $h(\mathbf{D_0}') + h(\mathbf{D_1}') < h(\mathbf{D_0}) + h(\mathbf{D_1})$ or $\rho(A') < \rho(A)$, if $\rho(\mathbf{D_0}'),\rho(\mathbf{D_1}') < \rho(A')$, then there exists a proof tree $\mathbf{D}'$ with conclusion $[ \mathcal{S}' | \epsilon_{l'} ] \cup \mathcal{T}' \Rightarrow \Delta'$ such that $\rho(\mathbf{D}') < \rho(A')$.

We proceed by case analysis on the last rule in $\mathbf{D_0}$.

\begin{itemize}
	\item[($Ax$)] We have $\mathcal{S} = \epsilon | A$, $k = 0$ and the desired sequent should be of the form $[ \epsilon | A | \epsilon_l] \cup \mathcal{T} \Rightarrow \Delta$. $n-1$ applications of $Lc$ on $\mathbf{D_1}$ proves such sequent.
	
	\item[($Ta$)] $\mathbf{D_0}$ proves $\epsilon \Rightarrow \top$. $\mathcal{T} \Rightarrow \Delta$ is proved by $\mathbf{D_1}$.
	
	\item[($Ex$)] This won't happen.
	
	\item[($Lw$)] $\mathbf{D_0}$ proves $\mathcal{S} | \Gamma , B | \mathcal{R} \Rightarrow \nabla^k A$ and has a subproof $\mathbf{D_0}'$ of $\mathcal{S} | \Gamma | \mathcal{R} \Rightarrow \nabla^k A$.
	\begin{prooftree}
		\noLine
		\AXC{$\mathbf{D_0}'$}
		\UIC{$\mathcal{S} | \Gamma | \mathcal{R} \Rightarrow \nabla^k A$}
		\RightLabel{$Lw$}
		\UIC{$\mathcal{S} | \Gamma , B | \mathcal{R} \Rightarrow \nabla^k A$}

		
		\noLine
		\AXC{$\mathbf{D_1}$}
		\UIC{$\mathcal{T} \cup [A^n | \epsilon_{k+l}] \Rightarrow \Delta$}

		\dashedLine\RightLabel{$Cut$}
		\BIC{$[\mathcal{S} | \Gamma , B | \mathcal{R} | \epsilon_l] \cup \mathcal{T} \Rightarrow \Delta$}
	\end{prooftree}
	From the induction hypothesis for $\mathbf{D_0}'$ and $\mathbf{D_1}$, we have a proof of $[\mathcal{S} | \Gamma | \mathcal{R} | \epsilon_l] \cup \mathcal{T} \Rightarrow \Delta$ with rank lower than that of $A$. By applying $Lw$ in the proper place, we have $[\mathcal{S} | \Gamma , B | \mathcal{R} | \epsilon_l] \cup \mathcal{T} \Rightarrow \Delta$, without increasing the cut-rank.
	\begin{prooftree}
		\noLine
		\AXC{$\mathbf{D_0}'$}
		\UIC{$\mathcal{S} | \Gamma | \mathcal{R} \Rightarrow \nabla^k A$}
		
		\noLine
		\AXC{$\mathbf{D_1}$}
		\UIC{$\mathcal{T} \cup [A^n | \epsilon_{k+l}] \Rightarrow \Delta$}
		
		\RightLabel{IH}
		\BIC{$[\mathcal{S} | \Gamma | \mathcal{R} | \epsilon_l] \cup \mathcal{T} \Rightarrow \Delta$}
		
		\RightLabel{$Lw$}
		\UIC{ $[\mathcal{S} | \Gamma , B | \mathcal{R} | \epsilon_l] \cup \mathcal{T} \Rightarrow \Delta$}
	\end{prooftree}
	
	\item[($Lc$)] $\mathbf{D_0}$ proves $\mathcal{S} | \Gamma , B | \mathcal{R} \Rightarrow \nabla^k A$ and has a subproof $\mathbf{D_0}'$ of $\mathcal{S} | \Gamma , B , B | \mathcal{R} \Rightarrow \nabla^k A$.
	\begin{prooftree}
		\noLine
		\AXC{$\mathbf{D_0}'$}
		\UIC{$\mathcal{S} | \Gamma , B , B | \mathcal{R} \Rightarrow \nabla^k A$}
		\RightLabel{$Lc$}
		\UIC{$\mathcal{S} | \Gamma , B | \mathcal{R} \Rightarrow \nabla^k A$}
		
		
		\noLine
		\AXC{$\mathbf{D_1}$}
		\UIC{$\mathcal{T} \cup [A^n | \epsilon_{l+k}] \Rightarrow \Delta$}
		
		\dashedLine\RightLabel{$Cut$}
		\BIC{$[\mathcal{S} | \Gamma , B | \mathcal{R} | \epsilon_l] \cup \mathcal{T} \Rightarrow \Delta$}
	\end{prooftree}
	From the induction hypothesis for $\mathbf{D_0}'$ and $\mathbf{D_1}$, we have a proof of $[\mathcal{S} | \Gamma , B , B | \mathcal{R} | \epsilon_l] \cup \mathcal{T} \Rightarrow \Delta$ with rank lower than that of $A$. By applying $Lc$ in the proper place, we have $[\mathcal{S} | \Gamma , B | \mathcal{R} | \epsilon_l] \cup \mathcal{T} \Rightarrow \Delta$, without increasing the cut-rank.
	\begin{prooftree}
		\noLine
		\AXC{$\mathbf{D_0}'$}
		\UIC{$\mathcal{S} | \Gamma , B , B | \mathcal{R} \Rightarrow \nabla^k A$}
		
		\noLine
		\AXC{$\mathbf{D_1}$}
		\UIC{$\mathcal{T} \cup [A^n | \epsilon_{l+k}] \Rightarrow \Delta$}
		
		\RightLabel{IH}
		\BIC{$[\mathcal{S} | \Gamma , B , B | \mathcal{R} | \epsilon_l] \cup \mathcal{T} \Rightarrow \Delta$}
		
		\RightLabel{$Lc$}
		\UIC{$[\mathcal{S} | \Gamma , B | \mathcal{R} | \epsilon_l] \cup \mathcal{T} \Rightarrow \Delta$}
	\end{prooftree}
	
	\item[($L\land_1$)] $\mathbf{D_0}$ proves $\mathcal{S} | \Gamma , B \land C | \mathcal{R} \Rightarrow \nabla^k A$ and has a subproof $\mathbf{D_0}'$ of $\mathcal{S} | \Gamma , B | \mathcal{R} \Rightarrow \nabla^k A$.
	\begin{prooftree}
		\noLine
		\AXC{$\mathbf{D_0}'$}
		\UIC{$\mathcal{S} | \Gamma , B | \mathcal{R} \Rightarrow \nabla^k A$}
		\UIC{$\mathcal{S} | \Gamma , B \land C | \mathcal{R} \Rightarrow \nabla^k A$}
		
		
		\noLine
		\AXC{$\mathbf{D_1}$}
		\UIC{$\mathcal{T} \cup [A^n | \epsilon_{l+k}] \Rightarrow \Delta$}
		
		\dashedLine\RightLabel{$Cut$}
		\BIC{$[\mathcal{S} | \Gamma , B \land C | \mathcal{R} | \epsilon_l] \cup \mathcal{T} \Rightarrow \Delta$}
	\end{prooftree}
	From the induction hypothesis for $\mathbf{D_0}'$ and $\mathbf{D_1}$, we have a proof of $[\mathcal{S} | \Gamma , B | \mathcal{R} | \epsilon_l] \cup \mathcal{T} \Rightarrow \Delta$ with rank lower than that of $A$. By applying $L\land$ in the proper place, we have $[\mathcal{S} | \Gamma , B \land C | \mathcal{R} | \epsilon_l] \cup \mathcal{T} \Rightarrow \Delta$, without increasing the cut-rank.
	\begin{prooftree}
		\noLine
		\AXC{$\mathbf{D_0}'$}
		\UIC{$\mathcal{S} | \Gamma , B | \mathcal{R} \Rightarrow \nabla^k A$}
		
		\noLine
		\AXC{$\mathbf{D_1}$}
		\UIC{$\mathcal{T} \cup [A^n | \epsilon_{l+k}] \Rightarrow \Delta$}
		
		\RightLabel{IH}
		\BIC{$[\mathcal{S} | \Gamma , B | \mathcal{R} | \epsilon_l] \cup \mathcal{T} \Rightarrow \Delta$}
		
		\RightLabel{$L\land$}
		\UIC{$[\mathcal{S} | \Gamma , B \land C | \mathcal{R} | \epsilon_l] \cup \mathcal{T} \Rightarrow \Delta$}
	\end{prooftree}
	\item[($L\land_2$)] The other $L\land$ is the same.
	
	\item[($L\lor$)]  $\mathbf{D_0}$ proves $\mathcal{S} | \Gamma , B \lor C | \mathcal{R} \Rightarrow \nabla^k A$ and has subproofs $\mathbf{D_0}'$ of $\mathcal{S} | \Gamma , B | \mathcal{R} \Rightarrow \nabla^k A$ and $\mathbf{D_0}''$ of $\mathcal{S} | \Gamma , B | \mathcal{R} \Rightarrow \nabla^k A$.
	\begin{prooftree}
		\noLine
		\AXC{$\mathbf{D_0}'$}
		\UIC{$\mathcal{S} | \Gamma , B | \mathcal{R} \Rightarrow \nabla^k A$}
		\noLine
		\AXC{$\mathbf{D_0}''$}
		\UIC{$\mathcal{S} | \Gamma , B | \mathcal{R} \Rightarrow \nabla^k A$}
		\RightLabel{$L\lor$}
		\BIC{$\mathcal{S} | \Gamma , B \lor C | \mathcal{R} \Rightarrow \nabla^k A$}
		
		
		\noLine
		\AXC{$\mathbf{D_1}$}
		\UIC{$\mathcal{T} \cup [A^n | \epsilon_{l+k}] \Rightarrow \Delta$}
		
		\dashedLine\RightLabel{$Cut$}
		\BIC{$[\mathcal{S} | \Gamma , B \lor C | \mathcal{R} | \epsilon_l] \cup \mathcal{T} \Rightarrow \Delta$}
	\end{prooftree}
	From the induction hypothesis for $\mathbf{D_0}'$ and $\mathbf{D_1}$, we have a proof of $[\mathcal{S} | \Gamma , B | \mathcal{R} | \epsilon_l] \cup \mathcal{T} \Rightarrow \Delta$ with rank lower than that of $A$. Also from the induction hypothesis for $\mathbf{D_0}''$ and $\mathbf{D_1}$, we have a proof of $[\mathcal{S} | \Gamma , C | \mathcal{R} | \epsilon_l] \cup \mathcal{T} \Rightarrow \Delta$ with rank lower than that of $A$. By applying $L\lor$ in the proper place, we have $[\mathcal{S} | \Gamma , B \lor C | \mathcal{R} | \epsilon_l] \cup \mathcal{T} \Rightarrow \Delta$, without increasing the cut-rank.
	\begin{prooftree}
		\noLine
		\AXC{$\mathbf{D_0}'$}
		\UIC{$\mathcal{S} | \Gamma , B | \mathcal{R} \Rightarrow \nabla^k A$}
		
		\noLine
		\AXC{$\mathbf{D_1}$}
		\UIC{$\mathcal{T} \cup [A^n | \epsilon_{l+k}] \Rightarrow \Delta$}
		
		\RightLabel{IH}
		\BIC{$[\mathcal{S} | \Gamma , B | \mathcal{R} | \epsilon_l] \cup \mathcal{T} \Rightarrow \Delta$}
		
		\noLine
		\AXC{$\mathbf{D_0}''$}
		\UIC{$\mathcal{S} | \Gamma , C | \mathcal{R} \Rightarrow \nabla^k A$}
		
		\noLine
		\AXC{$\mathbf{D_1}$}
		\UIC{$\mathcal{T} \cup [A^n | \epsilon_{l+k}] \Rightarrow \Delta$}
		
		\RightLabel{IH}
		\BIC{$[\mathcal{S} | \Gamma , C | \mathcal{R} | \epsilon_l] \cup \mathcal{T} \Rightarrow \Delta$}
		
		\RightLabel{$L\lor$}
		\BIC{$[\mathcal{S} | \Gamma , B \lor C | \mathcal{R} | \epsilon_l] \cup \mathcal{T} \Rightarrow \Delta$}
	\end{prooftree}
	
	\item[($L\nabla$)] $\mathbf{D_0}$ proves $\mathcal{S} | \Gamma | \Sigma , \nabla B | \mathcal{R} \Rightarrow \nabla^k A$ and has a subproof $\mathbf{D_0}'$ of $\mathcal{S} | \Gamma , B | \Sigma | \mathcal{R} \Rightarrow \nabla^k A$.
	\begin{prooftree}
		\noLine
		\AXC{$\mathbf{D_0}'$}
		\UIC{$\mathcal{S} | \Gamma , B | \Sigma | \mathcal{R} \Rightarrow \nabla^k A$}
		\RightLabel{$L\nabla$}
		\UIC{$\mathcal{S} | \Gamma | \Sigma , \nabla B | \mathcal{R} \Rightarrow \nabla^k A$}

		\noLine
		\AXC{$\mathbf{D_1}$}
		\UIC{$\mathcal{T} \cup [A^n | \epsilon_{l+k}] \Rightarrow \Delta$}

		\dashedLine\RightLabel{$Cut$}
		\BIC{$[\mathcal{S} | \Gamma | \Sigma , \nabla B | \mathcal{R} | \epsilon_l] \cup \mathcal{T} \Rightarrow \Delta$}
	\end{prooftree}
	From the induction hypothesis for $\mathbf{D_0}'$ and $\mathbf{D_1}$, we have a proof of $[\mathcal{S} | \Gamma , B | \Sigma | \mathcal{R} | \epsilon_l] \cup \mathcal{T} \Rightarrow \Delta$ with rank lower than that of $A$. By applying $L\nabla$ in the proper place, we have $[\mathcal{S} | \Gamma | \Sigma , \nabla B | \mathcal{R} | \epsilon_l] \cup \mathcal{T} \Rightarrow \Delta$, without increasing the cut-rank.
	\begin{prooftree}
		\noLine
		\AXC{$\mathbf{D_0}'$}
		\UIC{$\mathcal{S} | \Gamma , B | \Sigma | \mathcal{R} \Rightarrow \nabla^k A$}
		
		\noLine
		\AXC{$\mathbf{D_1}$}
		\UIC{$\mathcal{T} \cup [A^n | \epsilon_{l+k}] \Rightarrow \Delta$}
		
		\RightLabel{IH}
		\BIC{$[\mathcal{S} | \Gamma , B | \Sigma | \mathcal{R} | \epsilon_l] \cup \mathcal{T} \Rightarrow \Delta$}
		
		\RightLabel{$L\nabla$}
		\UIC{$[\mathcal{S} | \Gamma | \Sigma , \nabla B | \mathcal{R} | \epsilon_l] \cup \mathcal{T} \Rightarrow \Delta$}
	\end{prooftree}
	
	\item[($L\rightarrow$)] $\mathbf{D_0}$ proves $\mathcal{S} | \Gamma, B \rightarrow C | \Sigma | \mathcal{R} \Rightarrow \nabla^k A$ and has subproofs $\mathbf{D_0}'$ of $\mathcal{S} | \Gamma | \Sigma | \mathcal{R} \Rightarrow \nabla^{\#(\mathcal{R})} B$ and $\mathbf{D_0}''$ of $\mathcal{S} | \Gamma | \Sigma , C | \mathcal{R} \Rightarrow \nabla^k A$.
	\begin{prooftree}
		\noLine
		\AXC{$\mathbf{D_0}'$}
		\UIC{$\mathcal{S} | \Gamma | \Sigma | \mathcal{R} \Rightarrow \nabla^{\#(\mathcal{R})} B$}
		\noLine
		\AXC{$\mathbf{D_0}''$}
		\UIC{$\mathcal{S} | \Gamma | \Sigma , C | \mathcal{R} \Rightarrow \nabla^k A$}
		\RightLabel{$L\nabla$}
		\BIC{$\mathcal{S} | \Gamma, B \rightarrow C | \Sigma | \mathcal{R} \Rightarrow \nabla^k A$}
		
		
		\noLine
		\AXC{$\mathbf{D_1}$}
		\UIC{$\mathcal{T} \cup [A^n | \epsilon_{l+k}] \Rightarrow \Delta$}
		
		\dashedLine\RightLabel{$Cut$}
		\BIC{$[\mathcal{S} | \Gamma , B \rightarrow C | \Sigma | \mathcal{R} | \epsilon_l] \cup \mathcal{T} \Rightarrow \Delta$}
	\end{prooftree}
	From the induction hypothesis for $\mathbf{D_0}''$ and $\mathbf{D_1}$, we have a proof of
	$[\mathcal{S} | \Gamma | \Sigma , C | \mathcal{R} | \epsilon_l] \cup \mathcal{T} \Rightarrow \Delta$ with rank lower than that of $A$. Now in order to $L\rightarrow$ to be applicable on the resulting sequent and $\mathbf{D_0}'$, we must first identify their contexts. By $l$ times applications of $R\nabla$ and then $Lw$ with $\mathcal{T}$, we have $[\mathcal{S} | \Gamma | \Sigma | \mathcal{R} | \epsilon_l] \cup \mathcal{T} \Rightarrow \nabla^{\#(\mathcal{R})+l} B$. Then we can derive $[\mathcal{S} | \Gamma , B \rightarrow C | \Sigma | \mathcal{R} | \epsilon_l] \cup \mathcal{T} \Rightarrow \Delta$, from $L\rightarrow$ without increasing the cut-rank.
	\begin{prooftree}
		\noLine
		\AXC{$\mathbf{D_0}'$}
		\UIC{$\mathcal{S} | \Gamma | \Sigma | \mathcal{R} \Rightarrow \nabla^{\#(\mathcal{R})} B$}
		\doubleLine \RightLabel{$R\nabla$}
		\UIC{$\mathcal{S} | \Gamma | \Sigma | \mathcal{R} | \epsilon_l \Rightarrow \nabla^{\#(\mathcal{R})+l} B$}
		\doubleLine \RightLabel{$Lw$}
		\UIC{$[\mathcal{S} | \Gamma | \Sigma | \mathcal{R} | \epsilon_l] \cup \mathcal{T} \Rightarrow \nabla^{\#(\mathcal{R})+l} B$}
		
		\noLine
		\AXC{$\mathbf{D_0}''$}
		\UIC{$\mathcal{S} | \Gamma | \Sigma , C | \mathcal{R} \Rightarrow \nabla^k A$}
		\noLine
		\AXC{$\mathbf{D_1}$}
		\UIC{$\mathcal{T} \cup [A^n | \epsilon_{l+k}] \Rightarrow \Delta$}
		\RightLabel{IH}
		\BIC{$[\mathcal{S} | \Gamma | \Sigma , C | \mathcal{R} | \epsilon_l] \cup \mathcal{T} \Rightarrow \Delta$}
		
		\RightLabel{$L\rightarrow$}
		\BIC{$[\mathcal{S} | \Gamma , B \rightarrow C | \Sigma | \mathcal{R} | \epsilon_l] \cup \mathcal{T} \Rightarrow \Delta$}
	\end{prooftree}
	
	\item[($Rw$)] $\mathbf{D_0}$ proves $\mathcal{S} \Rightarrow \nabla^k A$ and has subproofs $\mathbf{D_0}'$ of $\mathcal{S} \Rightarrow$.
	\begin{prooftree}
		\noLine
		\AXC{$\mathbf{D_0}'$}
		\UIC{$\mathcal{S} \Rightarrow$}
		\RightLabel{$Rw$}
		\UIC{$\mathcal{S} \Rightarrow \nabla^k A$}
		
		\noLine
		\AXC{$\mathbf{D_1}$}
		\UIC{$\mathcal{T} \cup [A^n | \epsilon_{l+k}] \Rightarrow \Delta$}
		
		\dashedLine \RightLabel{$Cut$}
		\BIC{$[\mathcal{S} | \epsilon_l] \cup \mathcal{T} \Rightarrow \Delta$}
	\end{prooftree}
	$l$ times applications of $R\nabla$ on $\mathbf{D_0}'$ followed by proper $Lw$ and $Rw$ yields the desired sequent.
	\begin{prooftree}
		\noLine
		\AXC{$\mathbf{D_0}'$}
		\UIC{$\mathcal{S} \Rightarrow$}
		\doubleLine \RightLabel{$R\nabla$}
		\UIC{$\mathcal{S} | \epsilon_l \Rightarrow$}
		\RightLabel{$Lw$}
		\UIC{$[\mathcal{S} | \epsilon_l] \cup \mathcal{T} \Rightarrow$}
		\RightLabel{$Rw$}
		\UIC{$[\mathcal{S} | \epsilon_l] \cup \mathcal{T} \Rightarrow \Delta$}
	\end{prooftree}


	\item[($R*$)] In the cases that the last rule in $\mathbf{D_0}$ is any of the logical right-rules $R*$, its principal formula would be $\nabla^k A$. The only admissible rule where $k > 0$ would be $R\nabla$, so in other cases we assume $k = 0$. In each case, we will proceed by case analysis on the last rule of $\mathbf{D_1}$, but to avoid repeating similar cases, we will consider all cases in three groups: (I) Cases in which the last rule of $\mathbf{D_1}$ is any of the logical left-rules and (an instance of) $A$ is its principal formula, (II) $A$ is principal in $\mathbf{D_1}$, but the rule is structural and (III) other cases, that is, cases in which the cut-formula is not principal in the last rule of $\mathbf{D_1}$. Note that in (I), for any case of $\mathbf{D_0}$'s last rule, there is only one case in (I), but many different cases in (II) and (III). Also note that the cases in (II) and (III) are not dependent on the last rule of $\mathbf{D_0}$. The parens before each case show the last rule of $\mathbf{D_0}$ and $\mathbf{D_1}$ respectively.
	
	\begin{enumerate}[label=\Roman*]
		\item First, if the last rule in $\mathbf{D_1}$ is a logical left-rule and $A$ is also principal there. In 

		\begin{itemize}
			\item[$(R\land, L\land_1)$]‌
			\begin{prooftree}
				\noLine
				\AXC{$\mathbf{D_0}'$}
				\UIC{$\mathcal{S} \Rightarrow B$}
				\AXC{$\mathcal{S} \Rightarrow C$}
				\RightLabel{$R\land$}
				\BIC{$\mathcal{S} \Rightarrow B \land C$}
				
				\noLine
				\AXC{$\mathbf{D_1}'$}
				\UIC{$\mathcal{T} | \Gamma , (B \land C)^{n-1}, B | \mathcal{R} \Rightarrow \Delta$}
				\RightLabel{$L\land_1$}
				\UIC{$\mathcal{T} | \Gamma, (B \land C)^n | \mathcal{R} \Rightarrow \Delta$}
				
				\RightLabel{$Cut$} \dashedLine
				\BIC{$[ \mathcal{S} | \epsilon_{\#(\mathcal{R})} ] \cup [ \mathcal{T} | \Gamma | \mathcal{R} ] \Rightarrow \Delta$}
			\end{prooftree}
			Induction hypothesis for $\mathbf{D_0}$ and $\mathbf{D_0}'$ gives us $[ \mathcal{S} | \epsilon_{\#(\mathcal{R})} ] \cup [ \mathcal{T} | \Gamma , B | \mathcal{R} ] \Rightarrow \Delta$ with a lower cut-rank than $\rho(A)$. Again, applying induction hypothesis on this sequent and $\mathbf{D_1}'$ gives\\
			$[ \mathcal{S}^2 | \epsilon_{\#(\mathcal{R})} ] \cup [ \mathcal{T} | \Gamma | \mathcal{R} ] \Rightarrow \Delta$, which yields the desired sequent with enough applications of $Lc$.
			\begin{prooftree}
				\noLine
				\AXC{$\mathbf{D_0}'$}
				\UIC{$\mathcal{S} \Rightarrow B$}

				\noLine
				\AXC{$\mathbf{D_0}$}
				\UIC{$\mathcal{S} \Rightarrow B \land C$}
				\noLine
				\AXC{$\mathbf{D_1}'$}
				\UIC{$\mathcal{T} | \Gamma , (B \land C)^{n-1}, B | \mathcal{R} \Rightarrow \Delta$}
				
				\RightLabel{IH}
				\BIC{$[ \mathcal{S} | \epsilon_{\#(\mathcal{R})} ] \cup [ \mathcal{T} | \Gamma, B | \mathcal{R} ] \Rightarrow \Delta$}
	
				\RightLabel{IH}
				\BIC{$[ \mathcal{S}^2 | \epsilon_{\#(\mathcal{R})} ] \cup [ \mathcal{T} | \Gamma | \mathcal{R} ] \Rightarrow \Delta$}
				
				\doubleLine \RightLabel{$Lc$}
				\UIC{$[ \mathcal{S} | \epsilon_{\#(\mathcal{R})} ] \cup [ \mathcal{T} | \Gamma | \mathcal{R} ] \Rightarrow \Delta$}
			\end{prooftree}

			\item[$(R\land, L\land_2)$]‌
			\begin{prooftree}
				\AXC{$\mathcal{S} \Rightarrow B$}
				\noLine
				\AXC{$\mathbf{D_0}'$}
				\UIC{$\mathcal{S} \Rightarrow C$}
				\RightLabel{$R\land$}
				\BIC{$\mathcal{S} \Rightarrow B \land C$}
				
				\noLine
				\AXC{$\mathbf{D_1}'$}
				\UIC{$\mathcal{T} | \Gamma , (B \land C)^{n-1}, C | \mathcal{R} \Rightarrow \Delta$}
				\RightLabel{$L\land_2$}
				\UIC{$\mathcal{T} | \Gamma, (B \land C)^n | \mathcal{R} \Rightarrow \Delta$}
				
				\RightLabel{$Cut$} \dashedLine
				\BIC{$[ \mathcal{S} | \epsilon_{\#(\mathcal{R})} ] \cup [ \mathcal{T} | \Gamma | \mathcal{R} ] \Rightarrow \Delta$}
			\end{prooftree}
			Induction hypothesis for $\mathbf{D_0}$ and $\mathbf{D_0}'$ gives us $[ \mathcal{S} | \epsilon_{\#(\mathcal{R})} ] \cup [ \mathcal{T} | \Gamma , C | \mathcal{R} ] \Rightarrow \Delta$ with a lower cut-rank than $\rho(A)$. Again, applying induction hypothesis on this sequent and $\mathbf{D_0}'$ gives\\
			$[ \mathcal{S}^2 | \epsilon_{\#(\mathcal{R})} ] \cup [ \mathcal{T} | \Gamma | \mathcal{R} ] \Rightarrow \Delta$, which yields the desired sequent with enough applications of $Lc$.
			\begin{prooftree}
				\noLine
				\AXC{$\mathbf{D_0}'$}
				\UIC{$\mathcal{S} \Rightarrow C$}
				
				\noLine
				\AXC{$\mathbf{D_0}$}
				\UIC{$\mathcal{S} \Rightarrow B \land C$}
				\noLine
				\AXC{$\mathbf{D_1}'$}
				\UIC{$\mathcal{T} | \Gamma , (B \land C)^{n-1}, C | \mathcal{R} \Rightarrow \Delta$}
				
				\RightLabel{IH}
				\BIC{$[ \mathcal{S} | \epsilon_{\#(\mathcal{R})} ] \cup [ \mathcal{T} | \Gamma, C | \mathcal{R} ] \Rightarrow \Delta$}
				
				\RightLabel{IH}
				\BIC{$[ \mathcal{S}^2 | \epsilon_{\#(\mathcal{R})} ] \cup [ \mathcal{T} | \Gamma | \mathcal{R} ] \Rightarrow \Delta$}
				
				\doubleLine \RightLabel{$Lc$}
				\UIC{$[ \mathcal{S} | \epsilon_{\#(\mathcal{R})} ] \cup [ \mathcal{T} | \Gamma | \mathcal{R} ] \Rightarrow \Delta$}
			\end{prooftree}

			\item[$(R\lor_1, L\lor)$]‌
			\begin{prooftree}
				\noLine
				\AXC{$\mathbf{D_0}'$}
				\UIC{$\mathcal{S} \Rightarrow B$}
				\RightLabel{$R\lor_1$}
				\UIC{$\mathcal{S} \Rightarrow B \lor C$}

				\noLine
				\AXC{$\mathbf{D_1}'$}
				\UIC{$\mathcal{T} | \Gamma , (B \lor C)^{n-1} , B | \mathcal{R} \Rightarrow \Delta$}
				\AXC{$\mathcal{T} | \Gamma , (B \lor C)^{n-1} , C | \mathcal{R} \Rightarrow \Delta$}
				\RightLabel{$L\lor$}
				\BIC{$\mathcal{T} | \Gamma , (B \lor C)^n | \mathcal{R} \Rightarrow \Delta$}

				\RightLabel{$Cut$} \dashedLine
				\BIC{$[ \mathcal{S} | \epsilon_{\#(\mathcal{R})} ] \cup [ \mathcal{T} | \Gamma | \mathcal{R} ] \Rightarrow \Delta$}
			\end{prooftree}
			Induction hypothesis for $\mathbf{D_0}$ and $\mathbf{D_1}'$ gives us $[ \mathcal{S} | \epsilon_{\#(\mathcal{R})} ] \cup [ \mathcal{T} | \Gamma , B | \mathcal{R} ] \Rightarrow \Delta$ with a lower cut-rank than $\rho(A)$. Again, applying induction hypothesis on this sequent and $\mathbf{D_0}'$ gives\\
			$[ \mathcal{S}^2 | \epsilon_{\#(\mathcal{R})} ] \cup [ \mathcal{T} | \Gamma | \mathcal{R} ] \Rightarrow \Delta$, which yields the desired sequent with enough applications of $Lc$.
			\begin{prooftree}
				\noLine
				\AXC{$\mathbf{D_0}'$}
				\UIC{$\mathcal{S} \Rightarrow B$}

				\noLine
				\AXC{$\mathbf{D_0}$}
				\UIC{$\mathcal{S} \Rightarrow B \lor C$}

				\noLine
				\AXC{$\mathbf{D_1}'$}
				\UIC{$\mathcal{T} | \Gamma , (B \lor C)^{n-1} , B | \mathcal{R} \Rightarrow \Delta$}

				\RightLabel{IH}
				\BIC{$[ \mathcal{S} | \epsilon_{\#(\mathcal{R})} ] \cup [ \mathcal{T} | \Gamma , B | \mathcal{R} ] \Rightarrow \Delta$}
				
				\RightLabel{IH}
				\BIC{$[ \mathcal{S}^2 | \epsilon_{\#(\mathcal{R})} ] \cup [ \mathcal{T} | \Gamma | \mathcal{R} ] \Rightarrow \Delta$}
				
				\doubleLine \RightLabel{$Lc$}
				\UIC{$[ \mathcal{S} | \epsilon_{\#(\mathcal{R})} ] \cup [ \mathcal{T} | \Gamma | \mathcal{R} ] \Rightarrow \Delta$}
			\end{prooftree}

			\item[$(R\lor_2, L\lor)$]‌
			\begin{prooftree}
				\noLine
				\AXC{$\mathbf{D_0}'$}
				\UIC{$\mathcal{S} \Rightarrow C$}
				\RightLabel{$R\lor_2$}
				\UIC{$\mathcal{S} \Rightarrow B \lor C$}


				\AXC{$\mathcal{T} | \Gamma , (B \lor C)^{n-1} , B | \mathcal{R} \Rightarrow \Delta$}
				\noLine
				\AXC{$\mathbf{D_1}'$}
				\UIC{$\mathcal{T} | \Gamma , (B \lor C)^{n-1} , C | \mathcal{R} \Rightarrow \Delta$}
				\RightLabel{$L\lor$}
				\BIC{$\mathcal{T} | \Gamma , (B \lor C)^n | \mathcal{R} \Rightarrow \Delta$}
				
				\RightLabel{$Cut$} \dashedLine
				\BIC{$[ \mathcal{S} | \epsilon_{\#(\mathcal{R})} ] \cup [ \mathcal{T} | \Gamma | \mathcal{R} ] \Rightarrow \Delta$}
			\end{prooftree}
			Induction hypothesis for $\mathbf{D_0}$ and $\mathbf{D_1}'$ gives us $[ \mathcal{S} | \epsilon_{\#(\mathcal{R})} ] \cup [ \mathcal{T} | \Gamma , (B \lor C)^{n-1} | \mathcal{R} ] \Rightarrow \Delta$ with a lower cut-rank than $\rho(A)$. Again, applying induction hypothesis on this sequent and $\mathbf{D_0}'$ gives 
			$[ \mathcal{S}^2 | \epsilon_{\#(\mathcal{R})} ] \cup [ \mathcal{T} | \Gamma | \mathcal{R} ] \Rightarrow \Delta$, which yields the desired sequent with enough applications of $Lc$.
			\begin{prooftree}
				\noLine
				\AXC{$\mathbf{D_0}'$}
				\UIC{$\mathcal{S} \Rightarrow C$}

				\noLine
				\AXC{$\mathbf{D_0}$}
				\UIC{$\mathcal{S} \Rightarrow B \lor C$}

				\noLine
				\AXC{$\mathbf{D_1}'$}
				\UIC{$\mathcal{T} | \Gamma , (B \lor C)^{n-1} , C | \mathcal{R} \Rightarrow \Delta$}
				
				\RightLabel{IH}
				\BIC{$[ \mathcal{S} | \epsilon_{\#(\mathcal{R})} ] \cup [ \mathcal{T} | \Gamma , C | \mathcal{R} ] \Rightarrow \Delta$}
				
				\RightLabel{IH}
				\BIC{$[ \mathcal{S}^2 | \epsilon_{\#(\mathcal{R})} ] \cup [ \mathcal{T} | \Gamma | \mathcal{R} ] \Rightarrow \Delta$}
				
				\doubleLine \RightLabel{$Lc$}
				\UIC{$[ \mathcal{S} | \epsilon_{\#(\mathcal{R})} ] \cup [ \mathcal{T} | \Gamma | \mathcal{R} ] \Rightarrow \Delta$}
			\end{prooftree}

			\item[$(R\nabla, L\nabla)$] In fact, this is the only case where $k$ can be more than $0$.
			\begin{prooftree}
				\noLine
				\AXC{$\mathbf{D_0}$}
				\UIC{$\mathcal{S} | \epsilon_1 \Rightarrow \nabla^{k+1} B$}
				
				\noLine
				\AXC{$\mathbf{D_1}'$}
				\UIC{$\mathcal{T} \cup [B | (\nabla B)^{n-1} | \epsilon_{l+k}] \Rightarrow \Delta$}
				\RightLabel{$L\nabla$}
				\UIC{$\mathcal{T} \cup [(\nabla B)^n | \epsilon_{l+k}] \Rightarrow \Delta$}
				
				\RightLabel{$Cut$} \dashedLine
				\BIC{$[ \mathcal{S} | \epsilon_{l+1} ] \cup \mathcal{T} \Rightarrow \Delta$}
			\end{prooftree}
			First apply induction hypothesis for $\mathbf{D_0}$ and $\mathbf{D_1}'$ with $A' := \nabla B$. Again apply the induction hypothesis on $\mathbf{D_0}$ and the resulting sequent, this time with $A' := B$.
			
			\begin{prooftree}
				\noLine
				\AXC{$\mathbf{D_0}$}
				\UIC{$\mathcal{S} | \epsilon_1 \Rightarrow \nabla^{k+1} B$}
				
				
				\noLine
				\AXC{$\mathbf{D_0}$}
				\UIC{$\mathcal{S} | \epsilon_1 \Rightarrow \nabla^{k+1} B$}
				
				\noLine
				\AXC{$\mathbf{D_1}'$}
				\UIC{$\mathcal{T} \cup [B | (\nabla B)^{n-1} | \epsilon_{l+k}] \Rightarrow \Delta$}
				
				\RightLabel{IH}
				\BIC{$[\mathcal{S} | \epsilon_{l+1}] \cup \mathcal{T} \cup [B | \epsilon_{l+k+1}] \Rightarrow \Delta$}
				
				
				\RightLabel{IH}
				\BIC{$[\mathcal{S}^2 | \epsilon_{l+1}] \cup \mathcal{T} \Rightarrow \Delta$}
				
				\RightLabel{$Lc$}
				\UIC{$[\mathcal{S} | \epsilon_{l+1}] \cup \mathcal{T} \Rightarrow \Delta$}
			\end{prooftree}


			\item[$(R\rightarrow, L\rightarrow)$]
			What we want: $[\mathcal{S} | \epsilon_{\#(\mathcal{R})+1}] \cup [\mathcal{T} | \Gamma | \Sigma | \mathcal{R}] \Rightarrow \Delta$.
			\begin{prooftree}
				\noLine
				\AXC{$\mathbf{D_0}'$}
				\UIC{$\mathcal{S} | B \Rightarrow C$}
				\RightLabel{$R\rightarrow$}
				\UIC{$\mathcal{S} \Rightarrow B \rightarrow C$}

				\noLine
				\AXC{$\mathbf{D_1}'$}
				\UIC{$\mathcal{T} | \Gamma , (B \rightarrow C)^{n-1} | \Sigma | \mathcal{R} \Rightarrow \nabla^{\#(\mathcal{R})} B$}
				\noLine
				\AXC{$\mathbf{D_1}''$}
				\UIC{$\mathcal{T} | \Gamma , (B \rightarrow C)^{n-1} | \Sigma , C | \mathcal{R} \Rightarrow \Delta$}
				\RightLabel{$L\rightarrow$}
				\BIC{$\mathcal{T} | \Gamma, (B \rightarrow C)^n | \Sigma | \mathcal{R} \Rightarrow \Delta$}
				
				\RightLabel{$Cut$} \dashedLine
				\BIC{$[\mathcal{S} | \epsilon_{\#(\mathcal{R})+1}] \cup [\mathcal{T} | \Gamma | \Sigma | \mathcal{R}] \Rightarrow \Delta$}
			\end{prooftree}
			From induction hypothesis for $\mathbf{D_0}$ and $\mathbf{D_1}'$ we have $[\mathcal{S} | \epsilon_{\#(\mathcal{R})+1}] \cup [\mathcal{T} | \Gamma | \Sigma | \mathcal{R}] \Rightarrow \nabla^{\#(\mathcal{R})} B$. Call it $\mathbf{D}'$.
			\begin{prooftree}
				\noLine
				\AXC{$\mathbf{D_0}$}
				\UIC{$\mathcal{S} \Rightarrow B \rightarrow C$}
				
				\noLine
				\AXC{$\mathbf{D_1}'$}
				\UIC{$\mathcal{T} | \Gamma , (B \rightarrow C)^{n-1} | \Sigma | \mathcal{R} \Rightarrow \nabla^{\#(\mathcal{R})} B$}
				
				\LeftLabel{$\mathbf{D}':~$}
				\RightLabel{IH}
				\BIC{$[\mathcal{S} | \epsilon_{\#(\mathcal{R})+1}] \cup [\mathcal{T} | \Gamma | \Sigma | \mathcal{R}] \Rightarrow \nabla^{\#(\mathcal{R})} B$}
			\end{prooftree}
			Again from IH for $\mathbf{D_0}$ and $\mathbf{D_1}''$ we have $[\mathcal{S} | \epsilon_{\#(\mathcal{R})+1}] \cup [\mathcal{T} | \Gamma | \Sigma , C | \mathcal{R}] \Rightarrow \Delta$. Call it $\mathbf{D}''$.
			\begin{prooftree}
				\noLine
				\AXC{$\mathbf{D_0}$}
				\UIC{$\mathcal{S} \Rightarrow B \rightarrow C$}
				
				\noLine
				\AXC{$\mathbf{D_1}''$}
				\UIC{$\mathcal{T} | \Gamma , (B \rightarrow C)^{n-1} | \Sigma , C | \mathcal{R} \Rightarrow \Delta$}
				
				\LeftLabel{$\mathbf{D}'':~$}
				\RightLabel{IH}
				\BIC{$[\mathcal{S} | \epsilon_{\#(\mathcal{R})+1}] \cup [\mathcal{T} | \Gamma | \Sigma , C | \mathcal{R}] \Rightarrow \Delta$}
			\end{prooftree}
			Now we use induction hypothesis on $\mathbf{D_0}'$ and $\mathbf{D}''$ to remove $C$, and another induction hypothesis with $\mathbf{D}'$, this time with $k' := \#(R)$, to remove $B$. Applying enough contractions, we can derive the desired sequent.
			\begin{prooftree}
				\noLine
				\AXC{$\mathbf{D}'$}
				\UIC{$[\mathcal{S} | \epsilon_{\#(\mathcal{R})+1}] \cup [\mathcal{T} | \Gamma | \Sigma | \mathcal{R}] \Rightarrow \nabla^{\#(\mathcal{R})} B$}


				\noLine
				\AXC{$\mathbf{D_0}'$}
				\UIC{$\mathcal{S} | B \Rightarrow C$}

				\noLine
				\AXC{$\mathbf{D}''$}
				\UIC{$[\mathcal{S} | \epsilon_{\#(\mathcal{R})+1}] \cup [\mathcal{T} | \Gamma | \Sigma , C | \mathcal{R}] \Rightarrow \Delta$}

				\RightLabel{IH}
				\BIC{$[\mathcal{S}^2 | B | \epsilon_{\#(\mathcal{R})}] \cup [\mathcal{T} | \Gamma | \Sigma | \mathcal{R}] \Rightarrow \Delta$}



				\RightLabel{IH}
				\BIC{$[\mathcal{S}^3 | \epsilon_{\#(\mathcal{R})}] \cup [\mathcal{T}^2 | \Gamma^2 | \Sigma^2 | \mathcal{R}^2] \Rightarrow \Delta$}



				\doubleLine \RightLabel{$Lc$}
				\UIC{$[\mathcal{S} | \epsilon_{\#(\mathcal{R})}] \cup [\mathcal{T} | \Gamma | \Sigma | \mathcal{R}] \Rightarrow \Delta$}
			\end{prooftree}

		\end{itemize}

		\item If $A$ is principal in the last rule of $\mathbf{D_1}$ and it is structural.
		\begin{itemize}
			\item[$(R*, Lw)$]‌
			\begin{prooftree}
				\noLine
				\AXC{$\mathbf{D_0}$}
				\UIC{$\mathcal{S} \Rightarrow \nabla^k A$}
				
				\noLine
				\AXC{$\mathbf{D_1}'$}
				\UIC{$\mathcal{T} \cup [A^{n-1} | \epsilon_{l+k}] \Rightarrow \Delta$}
				\RightLabel{$Lw$}
				\UIC{$\mathcal{T} \cup [A^n | \epsilon_{l+k}] \Rightarrow \Delta$}
				
				\dashedLine\RightLabel{$Cut$}
				\BIC{$[\mathcal{S} | \epsilon_l] \cup \mathcal{T} \Rightarrow \Delta$}
			\end{prooftree}
			By induction hypothesis for $\mathbf{D_0}$ and $\mathbf{D_1}'$ we have
			\begin{prooftree}
				\noLine
				\AXC{$\mathbf{D_0}$}
				\UIC{$\mathcal{S} \Rightarrow \nabla^k A$}
				
				\noLine
				\AXC{$\mathbf{D_1}'$}
				\UIC{$\mathcal{T} \cup [A^{n-1} | \epsilon_{l+k}] \Rightarrow \Delta$}
				
				\RightLabel{IH}
				\BIC{$[\mathcal{S} | \epsilon_l] \cup \mathcal{T}\Rightarrow \Delta$}
			\end{prooftree}
		
			\item[$(R*, Lc)$]‌
			\begin{prooftree}
				\noLine
				\AXC{$\mathbf{D_0}$}
				\UIC{$\mathcal{S} \Rightarrow \nabla^k A$}
				
				\noLine
				\AXC{$\mathbf{D_1}'$}
				\UIC{$\mathcal{T} \cup [A^{n+1} | \epsilon_{l+k}] \Rightarrow \Delta$}
				\RightLabel{$Lc$}
				\UIC{$\mathcal{T} \cup [A^n | \epsilon_{l+k}] \Rightarrow \Delta$}
				
				\dashedLine\RightLabel{$Cut$}
				\BIC{$[\mathcal{S} | \epsilon_l] \cup \mathcal{T} \Rightarrow \Delta$}
			\end{prooftree}
			By induction hypothesis for $\mathbf{D_0}$ and $\mathbf{D_1}'$ we have
			\begin{prooftree}
				\noLine
				\AXC{$\mathbf{D_0}$}
				\UIC{$\mathcal{S} \Rightarrow \nabla^k A$}
				
				\noLine
				\AXC{$\mathbf{D_1}'$}
				\UIC{$\mathcal{T} \cup [A^{n+1} | \epsilon_{l+k}] \Rightarrow \Delta$}
				
				\RightLabel{IH}
				\BIC{$[\mathcal{S} | \epsilon_l] \cup \mathcal{T} \Rightarrow \Delta$}
			\end{prooftree}
		\end{itemize}

		\item If $A$ is not principal in the last rule of $\mathbf{D_1}$.
		
		\begin{itemize}
			\item[$(R*, Ax)$] $k$ and $l$ have to be $0$, so $\mathbf{D_0}$ proves the desired sequent.
			
			\item[$(R*, Ta)$] Won't happen.
			
			\item[$(Rw, Ex)$] The last rule in $\mathbf{D_1}$ can be $Ex$ only in the case that $\mathbf{D_0}$ ends with $Rw$. So $\mathbf{D_0}$ already proves the desired sequent $\mathcal{S} \Rightarrow$.
			
			\item[$(R*, Lw)$]‌
			\begin{prooftree}
				\noLine
				\AXC{$\mathbf{D_0}$}
				\UIC{$\mathcal{S} \Rightarrow \nabla^k A$}

				\noLine
				\AXC{$\mathbf{D_1}'$}
				\UIC{$\mathcal{T} \cup [A^n | \epsilon_{l+k} ] \Rightarrow \Delta$}
				\RightLabel{$Lw$}
				\UIC{$\mathcal{T} \cup [A^n | \epsilon_{l+k}] \cup [B | \epsilon_r] \Rightarrow \Delta$}
				
				\dashedLine\RightLabel{$Cut$}
				\BIC{$[\mathcal{S} | \epsilon_l] \cup \mathcal{T} \cup [B | \epsilon_r] \Rightarrow \Delta$}
			\end{prooftree}
			By induction hypothesis for $\mathbf{D_0}$ and $\mathbf{D_1}'$ we have
			\begin{prooftree}
				\noLine
				\AXC{$\mathbf{D_0}$}
				\UIC{$\mathcal{S} \Rightarrow \nabla^k A$}
				
				\noLine
				\AXC{$\mathbf{D_1}'$}
				\UIC{$\mathcal{T} \cup [A^n | \epsilon_{l+k}] \Rightarrow \Delta$}
				\RightLabel{IH}
				\BIC{$[\mathcal{S} | \epsilon_l] \cup \mathcal{T} \Rightarrow \Delta$}
				
				\RightLabel{$Lw$}
				\UIC{$[\mathcal{S} | \epsilon_l] \cup \mathcal{T} \cup [B | \epsilon_r] \Rightarrow \Delta$}
			\end{prooftree}

			\item[$(R*, Rw)$]‌
			\begin{prooftree}
				\noLine
				\AXC{$\mathbf{D_0}$}
				\UIC{$\mathcal{S} \Rightarrow \nabla^k A$}
				
				\noLine
				\AXC{$\mathbf{D_1}'$}
				\UIC{$\mathcal{T} \cup [A^n | \epsilon_{l+k}] \Rightarrow$}
				\RightLabel{$Rw$}
				\UIC{$\mathcal{T} \cup [A^n | \epsilon_{l+k}] \Rightarrow B$}
				
				\dashedLine\RightLabel{$Cut$}
				\BIC{$[\mathcal{S} | \epsilon_l] \cup \mathcal{T} \Rightarrow B$}
			\end{prooftree}
			By induction hypothesis for $\mathbf{D_0}$ and $\mathbf{D_1}'$ we have
			\begin{prooftree}
				\noLine
				\AXC{$\mathbf{D_0}$}
				\UIC{$\mathcal{S} \Rightarrow \nabla^k A$}
				
				\noLine
				\AXC{$\mathbf{D_1}'$}
				\UIC{$\mathcal{T} \cup [A^n | \epsilon_{l+k}] \Rightarrow$}
				\RightLabel{IH}
				\BIC{$[\mathcal{S} | \epsilon_l] \cup \mathcal{T} \Rightarrow$}
				
				\RightLabel{$Rw$}
				\UIC{$[\mathcal{S} | \epsilon_l] \cup \mathcal{T} \Rightarrow B$}
			\end{prooftree}

			\item[$(R*, Lc)$]‌
			\begin{prooftree}
				\noLine
				\AXC{$\mathbf{D_0}$}
				\UIC{$\mathcal{S} \Rightarrow \nabla^k A$}

				\noLine
				\AXC{$\mathbf{D_1}'$}
				\UIC{$\mathcal{T} \cup [A^n | \epsilon_{l+k}] \cup [B , B | \epsilon_r ] \Rightarrow \Delta$}
				\RightLabel{$Lc$}
				\UIC{$\mathcal{T} \cup [A^n | \epsilon_{l+k}] \cup [B | \epsilon_r] \Rightarrow \Delta$}

				\dashedLine\RightLabel{$Cut$}
				\BIC{$[\mathcal{S} | \epsilon_l] \cup \mathcal{T} \cup [B | \epsilon_r] \Rightarrow \Delta$}
			\end{prooftree}
			By induction hypothesis for $\mathbf{D_0}$ and $\mathbf{D_1}'$ we have
			\begin{prooftree}
				\noLine
				\AXC{$\mathbf{D_0}$}
				\UIC{$\mathcal{S} \Rightarrow \nabla^k A$}
				
				\noLine
				\AXC{$\mathbf{D_1}'$}
				\UIC{$\mathcal{T} \cup [A^n | \epsilon_{l+k}] \cup [B , B | \epsilon_r ] \Rightarrow \Delta$}
				\RightLabel{IH}
				\BIC{$[\mathcal{S} | \epsilon_l] \cup \mathcal{T} \cup [B , B | \epsilon_r] \Rightarrow \Delta$}
				
				\RightLabel{$Lc$}
				\UIC{$[\mathcal{S} | \epsilon_l] \cup \mathcal{T} \cup [B | \epsilon_r] \Rightarrow \Delta$}
			\end{prooftree}
		
			\item[$(R*, L\land_1)$]‌
			\begin{prooftree}
				\noLine
				\AXC{$\mathbf{D_0}$}
				\UIC{$\mathcal{S} \Rightarrow \nabla^k A$}
				
				\noLine
				\AXC{$\mathbf{D_1}'$}
				\UIC{$\mathcal{T} [A^n | \epsilon_{l+k}] \cup [B | \epsilon_r] \Rightarrow \Delta$}
				\RightLabel{$L\land_1$}
				\UIC{$\mathcal{T} \cup [A^n | \epsilon_{l+k}] \cup [B \land C | \epsilon_r] \Rightarrow \Delta$}
				
				\dashedLine\RightLabel{$Cut$}
				\BIC{$[\mathcal{S} | \epsilon_l] \cup \mathcal{T} \cup [B \land C | \epsilon_r] \Rightarrow \Delta$}
			\end{prooftree}
			By induction hypothesis for $\mathbf{D_0}$ and $\mathbf{D_1}'$ we have
			\begin{prooftree}
				\noLine
				\AXC{$\mathbf{D_0}$}
				\UIC{$\mathcal{S} \Rightarrow \nabla^k A$}
				
				\noLine
				\AXC{$\mathbf{D_1}'$}
				\UIC{$\mathcal{T} [A^n | \epsilon_{l+k}] \cup [B | \epsilon_r] \Rightarrow \Delta$}
				\RightLabel{IH}
				\BIC{$[\mathcal{S} | \epsilon_l] \cup \mathcal{T} \cup [B | \epsilon_r] \Rightarrow \Delta$}
				
				\RightLabel{$L\land_1$}
				\UIC{$[\mathcal{S} | \epsilon_l] \cup \mathcal{T} \cup [B \land C | \epsilon_r] \Rightarrow \Delta$}
			\end{prooftree}

			\item[$(R*, L\land_2)$]‌
			\begin{prooftree}
				\noLine
				\AXC{$\mathbf{D_0}$}
				\UIC{$\mathcal{S} \Rightarrow \nabla^k A$}
				
				\noLine
				\AXC{$\mathbf{D_1}'$}
				\UIC{$\mathcal{T} [A^n | \epsilon_{l+k}] \cup [C | \epsilon_r] \Rightarrow \Delta$}
				\RightLabel{$L\land_2$}
				\UIC{$\mathcal{T} \cup [A^n | \epsilon_{l+k}] \cup [B \land C | \epsilon_r] \Rightarrow \Delta$}
				
				\dashedLine\RightLabel{$Cut$}
				\BIC{$[\mathcal{S} | \epsilon_l] \cup \mathcal{T} \cup [B \land C | \epsilon_r] \Rightarrow \Delta$}
			\end{prooftree}
			By induction hypothesis for $\mathbf{D_0}$ and $\mathbf{D_1}'$ we have
			\begin{prooftree}
				\noLine
				\AXC{$\mathbf{D_0}$}
				\UIC{$\mathcal{S} \Rightarrow \nabla^k A$}
				
				\noLine
				\AXC{$\mathbf{D_1}'$}
				\UIC{$\mathcal{T} [A^n | \epsilon_{l+k}] \cup [C | \epsilon_r] \Rightarrow \Delta$}
				\RightLabel{IH}
				\BIC{$[\mathcal{S} | \epsilon_l] \cup \mathcal{T} \cup [C | \epsilon_r] \Rightarrow \Delta$}
				
				\RightLabel{$L\land_2$}
				\UIC{$[\mathcal{S} | \epsilon_l] \cup \mathcal{T} \cup [B \land C | \epsilon_r] \Rightarrow \Delta$}
			\end{prooftree}

			\item[$(R*, R\land)$]‌
			\begin{prooftree}
				\noLine
				\AXC{$\mathbf{D_0}$}
				\UIC{$\mathcal{S} \Rightarrow \nabla^k A$}
				
				\noLine
				\AXC{$\mathbf{D_1}'$}
				\UIC{$\mathcal{T} \cup [A^n | \epsilon_{l+k}] \Rightarrow B$}
				\noLine
				\AXC{$\mathbf{D_1}''$}
				\UIC{$\mathcal{T} \cup [A^n | \epsilon_{l+k}] \Rightarrow C$}
				\RightLabel{$R\land$}
				\BIC{$\mathcal{T} \cup [A^n | \epsilon_{l+k}] \Rightarrow B \land C$}
				
				\dashedLine\RightLabel{$Cut$}
				\BIC{$[\mathcal{S} | \epsilon_l] \cup \mathcal{T} \Rightarrow B \land C$}
			\end{prooftree}
			By induction hypothesis, once for $\mathbf{D_0}$ and $\mathbf{D_1}'$ and again for $\mathbf{D_0}$ and $\mathbf{D_1}''$
			\begin{prooftree}
				\noLine
				\AXC{$\mathbf{D_0}$}
				\UIC{$\mathcal{S} \Rightarrow \nabla^k A$}
				
				\noLine
				\AXC{$\mathbf{D_1}'$}
				\UIC{$\mathcal{T} \cup [A^n | \epsilon_{l+k}] \Rightarrow B$}
				
				\RightLabel{IH}
				\BIC{$[\mathcal{S} | \epsilon_l] \cup \mathcal{T} \Rightarrow B$}
				
				\noLine
				\AXC{$\mathbf{D_0}$}
				\UIC{$\mathcal{S} \Rightarrow A$}
				
				\noLine
				\AXC{$\mathbf{D_1}''$}
				\UIC{$\mathcal{T} \cup [A^n | \epsilon_{l+k}] \Rightarrow C$}
				
				\RightLabel{IH}
				\BIC{$[\mathcal{S} | \epsilon_l] \cup \mathcal{T} \Rightarrow C$}
				
				\RightLabel{$R\land$}
				\BIC{$[\mathcal{S} | \epsilon_l] \cup \mathcal{T} \Rightarrow B \land C$}
			\end{prooftree}

			\item[$(R*, L\lor)$]‌
			\begin{prooftree}
				\noLine
				\AXC{$\mathbf{D_0}$}
				\UIC{$\mathcal{S} \Rightarrow \nabla^k A$}
				
				\noLine
				\AXC{$\mathbf{D_1}'$}
				\UIC{$\mathcal{T} \cup [A^n | \epsilon_{l+k}] \cup [B | \epsilon_r] \Rightarrow \Delta$}
				\noLine
				\AXC{$\mathbf{D_1}''$}
				\UIC{$\mathcal{T} \cup [A^n | \epsilon_{l+k}] \cup [C | \epsilon_r] \Rightarrow \Delta$}
				\RightLabel{$L\lor$}
				\BIC{$\mathcal{T} \cup [A^n | \epsilon_{l+k}] \cup [B \lor C | \epsilon_r] \Rightarrow \Delta$}
				
				\dashedLine\RightLabel{$Cut$}
				\BIC{$[\mathcal{S} | \epsilon_l] \cup \mathcal{T} \cup [B \lor C | \epsilon_r] \Rightarrow \Delta$}
			\end{prooftree}
			By induction hypothesis, once for $\mathbf{D_0}$ and $\mathbf{D_1}'$ and again for $\mathbf{D_0}$ and $\mathbf{D_1}''$
			\begin{prooftree}
				\noLine
				\AXC{$\mathbf{D_0}$}
				\UIC{$\mathcal{S} \Rightarrow \nabla^k A$}
				
				\noLine
				\AXC{$\mathbf{D_1}'$}
				\UIC{$\mathcal{T} \cup [A^n | \epsilon_{l+k}] \cup [B | \epsilon_r] \Rightarrow \Delta$}
				
				\RightLabel{IH}
				\BIC{$[\mathcal{S} | \epsilon_l] \cup \mathcal{T} \cup [B | \epsilon_r] \Rightarrow \Delta$}

				\noLine
				\AXC{$\mathbf{D_0}$}
				\UIC{$\mathcal{S} \Rightarrow \nabla^k A$}
				
				\noLine
				\AXC{$\mathbf{D_1}''$}
				\UIC{$\mathcal{T} \cup [A^n | \epsilon_{l+k}] \cup [C | \epsilon_r] \Rightarrow \Delta$}
				
				\RightLabel{IH}
				\BIC{$[\mathcal{S} | \epsilon_l] \cup \mathcal{T} \cup [C | \epsilon_r] \Rightarrow \Delta$}

				\RightLabel{$L\lor$}
				\BIC{$[\mathcal{S} | \epsilon_l] \cup \mathcal{T} \cup [B \lor C | \epsilon_r] \Rightarrow \Delta$}
			\end{prooftree}

			\item[$(R*, R\lor_1)$]‌
			\begin{prooftree}
				\noLine
				\AXC{$\mathbf{D_0}$}
				\UIC{$\mathcal{S} \Rightarrow \nabla^k A$}

				\noLine
				\AXC{$\mathbf{D_1}'$}
				\UIC{$\mathcal{T} \cup [A^n | \epsilon_{l+k}] \Rightarrow B$}
				\RightLabel{$R\lor_1$}
				\UIC{$\mathcal{T} \cup [A^n | \epsilon_{l+k}] \Rightarrow B \lor C$}

				\dashedLine\RightLabel{$Cut$}
				\BIC{$[\mathcal{S} | \epsilon_l] \cup \mathcal{T} \Rightarrow B \lor C$}
			\end{prooftree}
			By induction hypothesis for $\mathbf{D_0}$ and $\mathbf{D_1}'$
			\begin{prooftree}
				\noLine
				\AXC{$\mathbf{D_0}$}
				\UIC{$\mathcal{S} \Rightarrow \nabla^k A$}

				\noLine
				\AXC{$\mathbf{D_1}'$}
				\UIC{$\mathcal{T} \cup [A^n | \epsilon_{l+k}] \Rightarrow B$}
				\RightLabel{IH}
				\BIC{$[\mathcal{S} | \epsilon_l] \cup \mathcal{T} \Rightarrow B$}

				\RightLabel{$R\lor_1$}
				\UIC{$[\mathcal{S} | \epsilon_l] \cup \mathcal{T} \Rightarrow B \lor C$}
			\end{prooftree}

			\item[$(R*, R\lor_2)$]‌
			\begin{prooftree}
				\noLine
				\AXC{$\mathbf{D_0}$}
				\UIC{$\mathcal{S} \Rightarrow \nabla^k A$}
				
				\noLine
				\AXC{$\mathbf{D_1}'$}
				\UIC{$\mathcal{T} \cup [A^n | \epsilon_{l+k}] \Rightarrow C$}
				\RightLabel{$R\lor_1$}
				\UIC{$\mathcal{T} \cup [A^n | \epsilon_{l+k}] \Rightarrow B \lor C$}
				
				\dashedLine\RightLabel{$Cut$}
				\BIC{$[\mathcal{S} | \epsilon_l] \cup \mathcal{T} \Rightarrow B \lor C$}
			\end{prooftree}
			By induction hypothesis for $\mathbf{D_0}$ and $\mathbf{D_1}'$
			\begin{prooftree}
				\noLine
				\AXC{$\mathbf{D_0}$}
				\UIC{$\mathcal{S} \Rightarrow \nabla^k A$}
				
				\noLine
				\AXC{$\mathbf{D_1}'$}
				\UIC{$\mathcal{T} \cup [A^n | \epsilon_{l+k}] \Rightarrow C$}
				\RightLabel{IH}
				\BIC{$[\mathcal{S} | \epsilon_l] \cup \mathcal{T} \Rightarrow C$}
				
				\RightLabel{$R\lor_1$}
				\UIC{$[\mathcal{S} | \epsilon_l] \cup \mathcal{T} \Rightarrow B \lor C$}
			\end{prooftree}

			\item[$(R*, L\rightarrow)$]‌
			\begin{prooftree}
				\noLine
				\AXC{$\mathbf{D_0}$}
				\UIC{$\mathcal{S} \Rightarrow \nabla^k A$}


				\noLine
				\AXC{$\mathbf{D_1}'$}
				\UIC{$\mathcal{T} \cup [A^n | \epsilon_{l+k}] \Rightarrow \nabla^r B$}
				
				\noLine
				\AXC{$\mathbf{D_1}''$}
				\UIC{$\mathcal{T} \cup [A^n | \epsilon_{l+k}] \cup [C | \epsilon_r] \Rightarrow \Delta$}
				
				\RightLabel{$L\rightarrow$}
				\BIC{$\mathcal{T} \cup [A^n | \epsilon_{l+k}] \cup [B \rightarrow C | \epsilon_{r+1}] \Rightarrow \Delta$}


				\dashedLine\RightLabel{$Cut$}
				\BIC{$[\mathcal{S} | \epsilon_l] \cup \mathcal{T} \cup [B \rightarrow C | \epsilon_{r+1}] \Rightarrow \Delta$}
			\end{prooftree}
			By induction hypothesis, once for $\mathbf{D_0}$ and $\mathbf{D_1}'$ and again for $\mathbf{D_0}$ and $\mathbf{D_1}''$
			\begin{prooftree}
				\noLine
				\AXC{$\mathbf{D_0}$}
				\UIC{$\mathcal{S} \Rightarrow \nabla^k A$}
				
				\noLine
				\AXC{$\mathbf{D_1}'$}
				\UIC{$\mathcal{T} \cup [A^n | \epsilon_{l+k}] \Rightarrow \nabla^r B$}
				
				\RightLabel{IH}
				\BIC{$[\mathcal{S} | \epsilon_l] \cup \mathcal{T} \Rightarrow \nabla^r B$}
				
				\noLine
				\AXC{$\mathbf{D_0}$}
				\UIC{$\mathcal{S} \Rightarrow A$}
				
				\noLine
				\AXC{$\mathbf{D_1}''$}
				\UIC{$\mathcal{T} \cup [A^n | \epsilon_{l+k}] \cup [C | \epsilon_r] \Rightarrow \Delta$}
				
				\RightLabel{IH}
				\BIC{$[\mathcal{S} | \epsilon_l] \cup \mathcal{T} \cup [\epsilon | C | \epsilon_r] \Rightarrow \Delta$}
				
				\RightLabel{$L\rightarrow$}
				\BIC{$[\mathcal{S} | \epsilon_l] \cup \mathcal{T} \cup [B \rightarrow C | \epsilon_{r+1}] \Rightarrow \Delta$}
			\end{prooftree}

			\item[$(R*, R\rightarrow)$]‌
			\begin{prooftree}
				\noLine
				\AXC{$\mathbf{D_0}$}
				\UIC{$\mathcal{S} \Rightarrow \nabla^k A$}
				
				\noLine
				\AXC{$\mathbf{D_1}'$}
				\UIC{$[\mathcal{T} | B] \cup [A^n | \epsilon_{l+k+1}] \Rightarrow C$}
				\RightLabel{$R\rightarrow$}
				\UIC{$\mathcal{T} \cup [A^n | \epsilon_{l+k}] \Rightarrow B \rightarrow C$}
				
				\dashedLine\RightLabel{$Cut$}
				\BIC{$[\mathcal{S} | \epsilon_l] \cup \mathcal{T} \Rightarrow B \rightarrow C$}
			\end{prooftree}
			By induction hypothesis for $\mathbf{D_0}$ and $\mathbf{D_1}'$
			\begin{prooftree}
				\noLine
				\AXC{$\mathbf{D_0}$}
				\UIC{$\mathcal{S} \Rightarrow \nabla^k A$}
				
				\noLine
				\AXC{$\mathbf{D_1}'$}
				\UIC{$[\mathcal{T} | B] \cup [A^n | \epsilon_{l+k+1}] \Rightarrow C$}
				\RightLabel{IH}
				\BIC{$[\mathcal{S} | \epsilon_{l+1}] \cup [\mathcal{T} | B] \Rightarrow C$}
				
				\RightLabel{$R\rightarrow$}
				\UIC{$[\mathcal{S} | \epsilon_l] \cup \mathcal{T} \Rightarrow B \rightarrow C$}
			\end{prooftree}
		
			\item[$(R*, L\nabla)$]‌
			\begin{prooftree}
				\noLine
				\AXC{$\mathbf{D_0}$}
				\UIC{$\mathcal{S} \Rightarrow \nabla^k A$}
				
				\noLine
				\AXC{$\mathbf{D_1}'$}
				\UIC{$\mathcal{T} \cup [A^n | \epsilon_{l+k}] \cup [B | \epsilon_{r+1}] \Rightarrow \Delta$}
				\RightLabel{$L\nabla$}
				\UIC{$\mathcal{T} \cup [A^n | \epsilon_{l+k}] \cup [\nabla B | \epsilon_r] \Rightarrow \Delta$}
				
				\dashedLine\RightLabel{$Cut$}
				\BIC{$[\mathcal{S} | \epsilon_l] \cup \mathcal{T} \cup [\nabla B | \epsilon_r] \Rightarrow \Delta$}
			\end{prooftree}
			By induction hypothesis for $\mathbf{D_0}$ and $\mathbf{D_1}'$
			\begin{prooftree}
				\noLine
				\AXC{$\mathbf{D_0}$}
				\UIC{$\mathcal{S} \Rightarrow \nabla^k A$}

				\noLine
				\AXC{$\mathbf{D_1}'$}
				\UIC{$\mathcal{T} \cup [A^n | \epsilon_{l+k}] \cup [B | \epsilon_{r+1}] \Rightarrow \Delta$}
				\RightLabel{IH}
				\BIC{$[\mathcal{S} | \epsilon_l] \cup \mathcal{T} \cup [B | \epsilon_{r+1}] \Rightarrow \Delta$}

				\RightLabel{$L\nabla$}
				\UIC{$[\mathcal{S} | \epsilon_l] \cup \mathcal{T} \cup [\nabla B | \epsilon_r] \Rightarrow \Delta$}
			\end{prooftree}

			\item[$(R*, R\nabla)$]‌
			\begin{prooftree}
				\noLine
				\AXC{$\mathbf{D_0}$}
				\UIC{$\mathcal{S} \Rightarrow \nabla^k A$}

				\noLine
				\AXC{$\mathbf{D_1}'$}
				\UIC{$\mathcal{T} \cup [A^n | \epsilon_{l+k}] \Rightarrow B$}
				\RightLabel{$R\nabla$}
				\UIC{$[\mathcal{T} | \epsilon_1] \cup [A^n | \epsilon_{l+k+1}] \Rightarrow \nabla B$}

				\dashedLine\RightLabel{$Cut$}
				\BIC{$[\mathcal{S} | \epsilon_{l+1}] \cup [\mathcal{T} | \epsilon_1] \Rightarrow \nabla B$}
			\end{prooftree}
			By induction hypothesis for $\mathbf{D_0}$ and $\mathbf{D_1}'$
			\begin{prooftree}
				\noLine
				\AXC{$\mathbf{D_0}$}
				\UIC{$\mathcal{S} \Rightarrow \nabla^k A$}

				\noLine
				\AXC{$\mathbf{D_1}'$}
				\UIC{$\mathcal{T} \cup [A^n | \epsilon_{l+k}] \Rightarrow B$}

				\RightLabel{IH}
				\BIC{$[\mathcal{S} | \epsilon_l] \cup \mathcal{T} \Rightarrow B$}


				\RightLabel{$R\nabla$}
				\UIC{$[\mathcal{S} | \epsilon_{l+1}] \cup [\mathcal{T} | \epsilon_1] \Rightarrow \nabla B$}
			\end{prooftree}
		\end{itemize}
	\end{enumerate}
\end{itemize}

\section{Corollary} \emph{Cut Elimination for GSTL: }
If $\text{GSTL}^- + Cut \vdash \Gamma \Rightarrow \Delta$, then $\text{GSTL}^- \vdash \Gamma \Rightarrow \Delta$.

\emph{Proof:} It suffices to show that for any proof tree of $\Gamma \Rightarrow \Delta$ like $\mathbf{D}$, there is another proof of it with a lower cut-rank. Using induction on $h(\mathbf{D})$, the induction hypothesis states that for any proof of $\Gamma' \Rightarrow \Delta'$ like $\mathbf{D'}$ such that $h(\mathbf{D'}) < h(\mathbf{D})$, there is another proof of $\Gamma' \Rightarrow \Delta'$ like $\mathbf{D''}$ such that $\rho(\mathbf{D''}) < \rho(\mathbf{D'})$. Particularly for the immediate sub-trees of $\mathbf{D}$, this gives us sub-trees with lower cut-rank, which we call $\mathbf{D}_i$. We now consider two cases for the last rule of $\mathbf{D}$

\begin{enumerate}[label=\Roman*]
	\item If the last rule of $\mathbf{D}$ is of a lower rank than $\rho(\mathbf{D})$, i.e. the cut rule with the maximum rank is not the last rule in $\mathbf{D}$, then we can apply the same last rule on $\mathbf{D}_i$s and get a proof of $\Gamma \Rightarrow \Delta$ with a lower cut-rank.
	
	\item If the last rule of $\mathbf{D}$ is an instance of cut rule with a cut-formula of rank $\rho(\mathbf{D})$, then we can apply theorem \ref{cut-admis} to $\mathbf{D_0}$ and $\mathbf{D_1}$ to get the same cut with a lower rank.
\end{enumerate}

\end{document}