
\section{iSTL} We define iSTL by the following rules.‌\\
\textbf{Axioms}
\begin{multicols}{3}
	\begin{prooftree}
		\AXC{}
		\RightLabel{$Id$}
		\UIC{$A \Rightarrow A$}
	\end{prooftree}
\columnbreak
	\begin{prooftree}
		\AXC{}
		\RightLabel{$Ta$}
		\UIC{$\Rightarrow \top$}
	\end{prooftree}
\columnbreak
	\begin{prooftree}
		\AXC{}
		\RightLabel{$Ex$}
		\UIC{$\bot \Rightarrow$}
	\end{prooftree}
\end{multicols}

\noindent\textbf{Structural Rules}
\begin{multicols}{3}
	\begin{prooftree}
		\RightLabel{$Lw$}
		\AXC{$\Gamma \Rightarrow \Delta$}
		\UIC{$\Gamma , A \Rightarrow \Delta$}
	\end{prooftree}
	\columnbreak
	\begin{prooftree}
		\RightLabel{$Rw$}
		\AXC{$\Gamma \Rightarrow$}
		\UIC{$\Gamma \Rightarrow A$}
	\end{prooftree}
	\columnbreak
	\begin{prooftree}
		\RightLabel{$Lc$}
		\AXC{$\Gamma , A , A \Rightarrow \Delta$}
		\UIC{$\Gamma , A \Rightarrow \Delta$}
	\end{prooftree}
\end{multicols}

\noindent\textbf{Logical Rules}
\begin{multicols}{3}
	\begin{prooftree}
		\RightLabel{$L\land_1$}
		\AXC{$\Gamma , A \Rightarrow \Delta$}
		\UIC{$\Gamma , A \land B \Rightarrow \Delta$}
	\end{prooftree}
	\columnbreak
	\begin{prooftree}
		\RightLabel{$L\land_2$}
		\AXC{$\Gamma , B \Rightarrow \Delta$}
		\UIC{$\Gamma , A \land B \Rightarrow \Delta$}
	\end{prooftree}
	\columnbreak
	\begin{prooftree}
		\RightLabel{$R\land$}
		\AXC{$\Gamma \Rightarrow A$}
		\AXC{$\Gamma \Rightarrow B$}
		\BIC{$\Gamma \Rightarrow A \land B$}
	\end{prooftree}
\end{multicols}
‌\\
\begin{multicols}{3}
	\begin{prooftree}
		\RightLabel{$L\lor$}
		\AXC{$\Gamma , A \Rightarrow \Delta$}
		\AXC{$\Gamma , B \Rightarrow \Delta$}
		\BIC{$\Gamma , A \lor B \Rightarrow \Delta$}
	\end{prooftree}
	\columnbreak
	\begin{prooftree}
		\RightLabel{$R\lor_1$}
		\AXC{$\Gamma \Rightarrow A$}
		\UIC{$\Gamma \Rightarrow A \lor B$}
	\end{prooftree}
	\columnbreak
	\begin{prooftree}
		\RightLabel{$R\lor_2$}
		\AXC{$\Gamma \Rightarrow B$}
		\UIC{$\Gamma \Rightarrow A \lor B$}
	\end{prooftree}
\end{multicols}
‌\\
\begin{multicols}{2}
	\begin{prooftree}
		\RightLabel{$L\rightarrow$}
		\AXC{$\Gamma \Rightarrow A$}
		\AXC{$\Gamma , B \Rightarrow \Delta$}
		\BIC{$\Gamma, \nabla(A \rightarrow B) \Rightarrow \Delta$}
	\end{prooftree}
	\columnbreak
	\begin{prooftree}
		\RightLabel{$R\rightarrow$}
		\AXC{$\nabla\Gamma , A \Rightarrow B$}
		\UIC{$\Gamma \Rightarrow A \rightarrow B$}
	\end{prooftree}
\end{multicols}
\noindent\textbf{Modal Rule}
\begin{prooftree}
	\RightLabel{$N$}
	\AXC{$\Gamma \Rightarrow A$}
	\UIC{$\nabla\Gamma \Rightarrow \nabla A$}
\end{prooftree}

\noindent\textbf{Cut}
\begin{prooftree}
	\RightLabel{$Cut$}
	\AXC{$\Gamma \Rightarrow A$}
	\AXC{$\Sigma , A \Rightarrow \Delta$}
	\BIC{$\Gamma , \Sigma \Rightarrow \Delta$}
\end{prooftree}

\subsection{Lemma}\label{lem:i-nabla-dist-and} For all $n > 0$, iSTL $\vdash \nabla^n (A \land B) \Rightarrow \nabla^n A \land \nabla^n B$

\textit{Proof}:
\begin{prooftree}
	\AXC{}
	\RightLabel{$Id$}
	\UIC{$A \Rightarrow A$}
	\RightLabel{$L\land_1$}
	\UIC{$A \land B \Rightarrow A$}
	\RightLabel{$N$} \doubleLine
	\UIC{$\nabla^n (A \land B) \Rightarrow \nabla^n A$}

	\AXC{}
	\RightLabel{$Id$}
	\UIC{$B \Rightarrow B$}
	\RightLabel{$L\land_2$}
	\UIC{$A \land B \Rightarrow B$}
	\RightLabel{$N$} \doubleLine	
	\UIC{$\nabla^n (A \land B) \Rightarrow \nabla^n B$}
	
	\RightLabel{$R\land$}
	\BIC{$\nabla^n (A \land B) \Rightarrow \nabla^n A \land \nabla^n B$}
\end{prooftree}

\subsection{Lemma}\label{lem:i-nabla-dist-or} iSTL $\vdash \nabla (A \lor B) \Rightarrow \nabla A \lor \nabla B$

\textit{Proof}:
\begin{prooftree}
	\AXC{}
	\RightLabel{$Id$}
	\UIC{$\nabla A \Rightarrow \nabla A$}
	\RightLabel{$R\lor_1$}
	\UIC{$\nabla A \Rightarrow \nabla A \lor \nabla B$}
	\RightLabel{$Lw$}
	\UIC{$\nabla A , \top \Rightarrow \nabla A \lor \nabla B$}
	\RightLabel{$R\rightarrow$}
	\UIC{$A \Rightarrow \top \rightarrow (\nabla A \lor \nabla B)$}

	\AXC{}
	\RightLabel{$Id$}
	\UIC{$\nabla B \Rightarrow \nabla B$}
	\RightLabel{$R\lor_2$}
	\UIC{$\nabla B \Rightarrow \nabla A \lor \nabla B$}
	\RightLabel{$Lw$}
	\UIC{$\nabla B , \top \Rightarrow \nabla A \lor \nabla B$}
	\RightLabel{$R\rightarrow$}
	\UIC{$B \Rightarrow \top \rightarrow (\nabla A \lor \nabla B)$}

	\RightLabel{$L\lor$}
	\BIC{$A \lor B \Rightarrow \top \rightarrow (\nabla A \lor \nabla B)$}
	\RightLabel{$N$}
	\UIC{$\nabla (A \lor B) \Rightarrow \nabla (\top \rightarrow (\nabla A \lor \nabla B))$}


	\AXC{}
	\RightLabel{$Ta$}
	\UIC{$\Rightarrow \top$}

	\AXC{}
	\RightLabel{$Id$}
	\UIC{$\nabla A \lor \nabla B \Rightarrow \nabla A \lor \nabla B$}

	\RightLabel{$L\rightarrow$}
	\BIC{$\nabla (\top \rightarrow (\nabla A \lor \nabla B)) \Rightarrow \nabla A \lor \nabla B$}



	\RightLabel{$Cut$}
	\BIC{$\nabla (A \lor B) \Rightarrow \nabla A \lor \nabla B$}
\end{prooftree}

\subsection{Lemma}\label{lem:i-nabla-n-dist-or} For all $n > 0$, iSTL $\vdash \nabla^n (A \lor B) \Rightarrow \nabla^n A \lor \nabla^n B$

\textit{Proof}: Let $\mathbf{D_1}$ be the proof of lemma \ref{lem:i-nabla-dist-or}, which proves $n = 1$ case. For $n > 1$

\begin{prooftree}
	\AXC{$\mathbf{D_{n-1}}$}
	\noLine
	\UIC{$\nabla^{n-1} (A \lor B) \Rightarrow \nabla^{n-1} A \lor \nabla^{n-1} B$}
	\RightLabel{$N$}
	\UIC{$\nabla^n (A \lor B) \Rightarrow \nabla (\nabla^{n-1} A \lor \nabla^{n-1} B)$}

	\AXC{$\mathbf{D_1}$}
	\noLine
	\UIC{$\nabla (\nabla^{n-1} A \lor \nabla^{n-1} B) \Rightarrow \nabla^n A \lor \nabla^n B$}
	
	\RightLabel{$Cut$} \LeftLabel{$\mathbf{D_n~:~~~~}$}
	\BIC{$\nabla^n (A \lor B) \Rightarrow \nabla^n A \lor \nabla^n B$}
\end{prooftree}

\subsection{Lemma}\label{lem:i-nabla-bot} iSTL $\vdash \nabla \bot \Rightarrow \bot$

\textit{Proof}:
\begin{prooftree}
	\AXC{}
	\RightLabel{$Ex$}
	\UIC{$\bot \Rightarrow$}
	\RightLabel{$Rw$}
	\UIC{$\bot \Rightarrow \top \rightarrow \bot$}
	\RightLabel{$N$}
	\UIC{$\nabla \bot \Rightarrow \nabla (\top \rightarrow \bot)$}

	\AXC{}
	\RightLabel{$Ta$}
	\UIC{$\Rightarrow \top$}	
	\AXC{}
	\RightLabel{$Id$}
	\UIC{$\bot \Rightarrow \bot$}
	\RightLabel{$L\rightarrow$}
	\BIC{$\nabla (\top \rightarrow \bot) \Rightarrow \bot$}
	
	\RightLabel{$Cut$}
	\BIC{$\nabla \bot \Rightarrow \bot$}
\end{prooftree}

\subsection{Lemma}\label{lem:i-nabla-n-bot} For $n \geq m > 0$, iSTL $\vdash \nabla^n \bot \Rightarrow \nabla^{n-m} \bot$.

\textit{Proof}: Let $\mathbf{D_1}$ be the proof of lemma \ref{lem:i-nabla-bot} which handles $n = m = 1$. By induction om $m$, let IH be the proof tree for $\nabla^n \bot \Rightarrow \nabla^{n-(m-1)} \bot$, which we have from the induction hypothesis. Then for $n > 1$
\begin{prooftree}
	\AXC{IH}
	\noLine
	\UIC{$\nabla^{n-m} \bot \Rightarrow \nabla^{n-(m-1)} \bot$}

	\AXC{$\mathbf{D_1}$}
	\noLine
	\UIC{$\nabla \bot \Rightarrow \bot$}
	\doubleLine \RightLabel{$N^{(n-m)}$}
	\UIC{$\nabla^{n-m+1} \bot \Rightarrow \nabla^{n-m} \bot$}

	\RightLabel{$Cut$}
	\BIC{$\nabla^n \bot \Rightarrow \nabla^{n-m} \bot$}
\end{prooftree}

\subsection{Lemma}\label{lem:i-nabla-dist-imp} For any $n > 0$, iSTL $\vdash \nabla^n (A \rightarrow B) \Rightarrow \nabla^n A \rightarrow \nabla^n B$

\textit{Proof}:
\begin{prooftree}
	\AXC{}
	\RightLabel{$Id$}
	\UIC{$A \Rightarrow A$}
	
	\AXC{}
	\RightLabel{$Id$}
	\UIC{$B \Rightarrow B$}
	\RightLabel{$Lw$}
	\UIC{$A , B \Rightarrow B$}
	
	\RightLabel{$L\rightarrow$}
	\BIC{$\nabla (A \rightarrow B) , A \Rightarrow B$}
	\RightLabel{$N$} \doubleLine
	\UIC{$\nabla^{n+1} (A \rightarrow B) , \nabla^n A \Rightarrow \nabla^n B$}
	\RightLabel{$R\rightarrow$}
	\UIC{$\nabla^n (A \rightarrow B) \Rightarrow \nabla^n A \rightarrow \nabla^n B$}
\end{prooftree}

\subsection{Lemma}\label{lem:modus-ponens} iSTL $\vdash A , \nabla (A \rightarrow B) \Rightarrow B$

\textit{Proof}:
\begin{prooftree}
	\AXC{}
	\RightLabel{$Id$}
	\UIC{$A \Rightarrow A$}

	\AXC{}
	\RightLabel{$Id$}
	\UIC{$B \Rightarrow B$}
	\RightLabel{$Lw$}
	\UIC{$A , B \Rightarrow B$}

	\RightLabel{$L \rightarrow$}
	\BIC{$A , \nabla (A \rightarrow B) \Rightarrow B$}
\end{prooftree}

\subsection{Lemma}\label{lem:impl-elim} If iSTL $\vdash \Rightarrow A \rightarrow B$ then iSTL $\vdash A \Rightarrow B$.

\textit{Proof}:
\begin{prooftree}
	\AXC{$\Rightarrow A \rightarrow B$}
	\RightLabel{$N$}
	\UIC{$\Rightarrow \nabla (A \rightarrow B)$}

	\AXC{}
	\RightLabel{\ref{lem:modus-ponens}}
	\UIC{$A, \nabla (A \rightarrow B) \Rightarrow B$}
	
	\RightLabel{$Cut$}
	\BIC{$A \Rightarrow B$}
\end{prooftree}

\subsection{Lemma}\label{lem:conj-context} For $n \geq 0$, iSTL $\vdash \{ A_i \}_{i=1}^n \Rightarrow \bigwedge_{i=1}^n A_i$

\textit{Proof}: For $n = 1$ we have $A_1 \Rightarrow A_1$ by $Id$. By induction on $n$, let IH be the proof tree for $\{ A_n \}_{i=1}^{n-1} \Rightarrow \bigwedge_{i=1}^{n-1}$, which we have from the induction hypothesis. For $n > 1$
\begin{prooftree}
	\AXC{IH}
	\noLine
	\UIC{$\{ A_i \}_{i=1}^{n-1} \Rightarrow \bigwedge_{i=1}^{n-1} A_i$}
	\RightLabel{$Lw$}
	\UIC{$\{ A_i \}_{i=1}^n \Rightarrow \bigwedge_{i=1}^{n-1} A_i$}

	\AXC{}
	\RightLabel{$Id$}
	\UIC{$A_n \Rightarrow A_n$}
	\doubleLine \RightLabel{$Lw$}
	\UIC{$\{ A_i \}_{i=1}^n \Rightarrow A_n$}

	\RightLabel{$R\land$}
	\BIC{$\{ A_i \}_{i=1}^n \Rightarrow \bigwedge_{i=1}^n A_i$}
\end{prooftree}