($R\rightarrow, L\rightarrow$)
		\begin{prooftree}
			\noLine
			\AXC{$\mathbf{D_0}'$}
			\UIC{$\nabla \Gamma , B \Rightarrow C$}
			\RightLabel{$R\rightarrow$}
			\UIC{$\Gamma \Rightarrow B \rightarrow C$}

			\noLine
			\AXC{$\mathbf{D_1}'$}
			\UIC{$\Sigma , (\nabla^{l+1} (B \rightarrow C))^{n-1} \Rightarrow \nabla^l B$}
			\noLine
			\AXC{$\mathbf{D_1}''$}
			\UIC{$\Sigma , (\nabla^{l+1} (B \rightarrow C))^{n-1} , \nabla^l C \Rightarrow \Delta$}
			\RightLabel{$L\rightarrow$}
			\BIC{$\Sigma , (\nabla^{l+1} (B \rightarrow C))^n \Rightarrow \Delta$}
			
			\RightLabel{$MC$} \dashedLine
			\BIC{$\nabla^{l+1} \Gamma , \Sigma \Rightarrow \Delta$}
		\end{prooftree}
		From induction hypothesis for $\mathbf{D_0}$ and $\mathbf{D_1}'$ we have $\nabla^{l+1} \Gamma , \Sigma \Rightarrow \nabla^l B$. Call it $\mathbf{D}'$.
		\begin{prooftree}
			\noLine
			\AXC{$\mathbf{D_0}$}
			\UIC{$\Gamma \Rightarrow B \rightarrow C$}
			
			\noLine
			\AXC{$\mathbf{D_1}'$}
			\UIC{$\Sigma , (\nabla^{l+1} (B \rightarrow C))^{n-1} \Rightarrow \nabla^l B$}
			
			\LeftLabel{$\mathbf{D}':~$}
			\RightLabel{IH}
			\BIC{$\nabla^{l+1} \Gamma , \Sigma \Rightarrow \nabla^l B$}
		\end{prooftree}
		Again from IH, this time for $\mathbf{D_0}$ and $\mathbf{D_1}''$ we have $\nabla^{l+1} \Gamma , \Sigma , \nabla^l C \Rightarrow \Delta$. Call it $\mathbf{D}''$.
		\begin{prooftree}
			\noLine
			\AXC{$\mathbf{D_0}$}
			\UIC{$\Gamma \Rightarrow B \rightarrow C$}
			
			\noLine
			\AXC{$\mathbf{D_1}''$}
			\UIC{$\Sigma , (\nabla^{l+1} (B \rightarrow C))^{n-1} , \nabla^l C \Rightarrow \Delta$}
			
			\LeftLabel{$\mathbf{D}'':~$}
			\RightLabel{IH}
			\BIC{$\nabla^{l+1} \Gamma , \Sigma , \nabla^l C \Rightarrow \Delta$}
		\end{prooftree}
		Cut $C$ from $\mathbf{D_0}'$ and $\mathbf{D}''$, then cut $\nabla^l B$ from the resulting sequent and $\mathbf{D}'$. Notice that $\nabla$ does not increase the rank of a formula, so $\rho(\nabla^l B) < \rho(B \rightarrow C)$. Applying enough contractions, we can derive the desired sequent.
		\begin{prooftree}
			\noLine
			\AXC{$\mathbf{D}'$}
			\UIC{$\nabla^{l+1} \Gamma , \Sigma \Rightarrow \nabla^l B$}


			\noLine
			\AXC{$\mathbf{D_0}'$}
			\UIC{$\nabla \Gamma , B \Rightarrow C$}

			\noLine
			\AXC{$\mathbf{D}''$}
			\UIC{$\nabla^{l+1} \Gamma , \Sigma , \nabla^l C \Rightarrow \Delta$}

			\RightLabel{$MC$}
			\BIC{$(\nabla^{l+1} \Gamma)^2 , \nabla^l B , \Sigma \Rightarrow \Delta$}



			\RightLabel{$MC$}
			\BIC{$(\nabla^{l+1} \Gamma)^3 , \Sigma^2 \Rightarrow \Delta$}



			\doubleLine \RightLabel{$Lc$}
			\UIC{$\nabla^{l+1} \Gamma , \Sigma \Rightarrow \Delta$}
		\end{prooftree}