\documentclass[12pt,a4paper]{article}
\input{preamble}

\begin{document}
    
\title{Interpolation for Logics of Spacetime}
\author[]{Amirhossein Akbar Tabatabai, Majid Alizadeh, Alireza Mahmoudian}
\affil[]{ }
\date{March 2, 2022}
\maketitle

\begin{abstract}
	A generalization of the notion of implication is introduced in \cite{amir}, as a binary operator which internalizes the reflexive and transitive properties of the provability order on the set of all propositions. This generalization gives rise to a classification of some sub-intuitionistic and sub-structural logics with various behaviors of their respecting implication operators. One of its specifications, which is called the logic of \emph{spacetime} in \cite{amir} makes a dynamic reading of the Proof Interpretation for conditional statements possible. This reading does not suffer from the well-known impredicativity in the BHK interpretation.

	In this paper, we will introduc a sequent-style calculus for the logic of spacetime, called $\stl$ along with an equivalent cut-free system, called $\gstl$. Then we will study some properties of thses systems such as subformula property, disjuction property, admissibility of the Visser's rule and existence of imterpolants.
\end{abstract}

\section{Introduction}
The usual interpretation of an intuitionistic proof for an implication is a structure that converts \emph{all} proofs of its antecedent to some proof for its consequent. This interpretation is impredicative in the sense that we are quantifying over the set of all proofs, while we are just defining some members of it, which are, the proofs for implication. The impredicativity of implication shows up more clearly when one is using a conditional assumption in an intuitionistic proof, which amounts to an application of the rule of \emph{modus ponens}. What this rule essentially says is that if we have a proof for an implication and a proof of its antecedent at the same time, then we can conclude its consequent.

The logic of spacetime remedies this by restricting the use of conditional assumption; So that the modus ponens rule in the logic of spacetime would not take a proof of conditional statement itself, but a proof of a modal operator, called $\nabla$, applied to the conditional statement. We can read this application of $\nabla$ as a \emph{delay} in use of implication, and interpret the proof of conditional statement as a function that converts all \emph{later} proofs of its antecedent to some \emph{later} proof for its consequent. So we can prove the consequent of a conditional statement, only if we have proved the conditional statement itself \emph{sooner} than the antecedent.\\

The logic of spacetime is represented by a sequent-style system called $\stl$ (known as $\istl(N)$\footnote{Note that in this paper $\istl$ is reserved for another system with intuitionistic implication.} in \cite{amir}), which has the same rules as the usual intuitionistic calculus $\mathbf{LJ}$, over the propositional language augumented with a unary connective $\nabla$, but with left and right implication rules replaced with the following rules, respectively.

\begin{multicols}{2}
	\begin{prooftree}
		\AXC{$\Gamma \Rightarrow A$}
		\AXC{$\Gamma, B \Rightarrow \Delta$}
		\RightLabel{$L \rightarrow$}
		\BIC{$\Gamma, \nabla (A \rightarrow B) \Rightarrow \Delta$}
	\end{prooftree}
	\columnbreak
	\begin{prooftree}
		\AXC{$\nabla \Gamma, A \Rightarrow B$}
		\RightLabel{$R \rightarrow$}
		\UIC{$\Gamma \Rightarrow A \rightarrow B$}
	\end{prooftree}
\end{multicols}
Furthermore, the system also has a rule to introduce $\nabla$ to both sides of a sequent.
\begin{prooftree}
	\AXC{$\Gamma \Rightarrow A$}
	\RightLabel{$N$}
	\UIC{$\nabla \Gamma \Rightarrow \nabla A$}
\end{prooftree}
So, generally, $\nabla (A \rightarrow B)$, and not $A \rightarrow B$, will be of use in proving $B$ from $A$.

In the next section of this paper, we will introduce a sequent style calculus for the spacetime logic, called $\stl$ and introduce an equivalent cut-free system $\gstl$, and then survey some extensions and their respecting semantics, including an extension of $\stl$ with a Heyting implication, called $\istl$, and simillarly, an equivalent cut-free system $\igstl$.
In the third section, the cut-elimination theorems for $\stl$ and its extensions will be proved. Then we will use this theorem to deduce important results about $\stl$ and its extensions, such as subformula property, disjuction property and admissibility of the Visser's rule.
And in the last section, we will show that some extensions of $\stl$ have interpolation property.

\section{Sequent calculi for the logics of spacetime}
In this section, will define the systems $\stl$ (defined as $\istl(N)$ in \cite{amir}) and $\gstl$, and show that these two systems are equivalent.
\begin{dfn}
	Consider the language $\mathcal{L}=\langle \wedge, \vee, \top, \bot, \nabla, \rightarrow, P \rangle$ where $P$ is the set of all atomic propositions. Define $\stl$ as the logic of the sequent-style system defined by the following rules, where in a sequent of the form $\Gamma \Rightarrow \Delta$, the left-hand side is a multiset of formulas $\Gamma$, and the right-hand side $\Delta$ is either a formula or empty.
\end{dfn}

\begin{flushleft}
 \textbf{Axioms:}
\end{flushleft}

\begin{multicols}{3}
	\begin{prooftree}
		\AXC{}
		\RightLabel{$Id$}
		\UIC{$ A \Rightarrow A$}
	\end{prooftree}
	\columnbreak
	\begin{prooftree}
		\AXC{}
		\RightLabel{$Ta$}
		\UIC{$ \Rightarrow \top$}
	\end{prooftree}
	\columnbreak
	\begin{prooftree}
		\AXC{}
		\RightLabel{$Ex$}
		\UIC{$ \bot \Rightarrow $}		
	\end{prooftree}
\end{multicols}

\begin{flushleft}
 		\textbf{Structural Rules:}
\end{flushleft}
\begin{multicols}{3}
	\begin{prooftree}
		\AXC{$ \Gamma \Rightarrow \Delta$}
		\RightLabel{$L w$}
		\UIC{$ \Gamma, A \Rightarrow \Delta$}
	\end{prooftree}
	\columnbreak
	\begin{prooftree}
		\AXC{$ \Gamma \Rightarrow $}
		\RightLabel{$R w$}
		 \UIC{$\Gamma \Rightarrow A$}		
	\end{prooftree}
	\columnbreak
	\begin{prooftree}
		\AXC{$ \Gamma, A, A \Rightarrow \Delta$}
		\RightLabel{$Lc$}
		\UIC{$\Gamma, A \Rightarrow \Delta$}		
	\end{prooftree}
\end{multicols}

\begin{flushleft}
 		\textbf{Cut:}
\end{flushleft}
\begin{center}
	\begin{prooftree}
		\AXC{$ \Gamma \Rightarrow A$}
		\AXC{$\Pi, A \Rightarrow \Delta$}
		\RightLabel{$cut$}
		\BIC{$ \Pi, \Gamma \Rightarrow \Delta$}
	\end{prooftree}
\end{center}

\begin{flushleft}
 \textbf{Conjunction Rules:}
\end{flushleft}
\begin{multicols}{3}
	\begin{prooftree}
		\AXC{$ \Gamma, A \Rightarrow \Delta$}
		\RightLabel{$L \wedge_1$}
		\UIC{$ \Gamma, A \wedge B \Rightarrow \Delta$}		
	\end{prooftree}
	\columnbreak
	\begin{prooftree}
		\AXC{$ \Gamma, B \Rightarrow \Delta$}
		\RightLabel{$L \wedge_2$}
		\UIC{$\Gamma, A \wedge B \Rightarrow \Delta$}		
	\end{prooftree}
	\columnbreak
	\begin{prooftree}
		\AXC{$\Gamma \Rightarrow A$}
		\AXC{$\Gamma \Rightarrow B$}
		\RightLabel{$R \wedge$}
		\BIC{$ \Gamma \Rightarrow A \wedge B $}		
	\end{prooftree}
\end{multicols}

\begin{flushleft}
 \textbf{Disjunction Rules:}
\end{flushleft}
\begin{multicols}{3}
	\begin{prooftree}
		\AXC{$ \Gamma, A \Rightarrow \Delta$}
		\AXC{$\Gamma, B \Rightarrow \Delta$}
		\RightLabel{$L \vee_1$}
		\BIC{$ \Gamma, A \vee B \Rightarrow \Delta$}		
	\end{prooftree}
	\columnbreak
	\begin{prooftree}
		\AXC{$\Gamma \Rightarrow A$}
		\RightLabel{$R \vee_2$}
		\UIC{$\Gamma \Rightarrow A \vee B$}		
	\end{prooftree}
	\columnbreak
	\begin{prooftree}
		\AXC{$\Gamma \Rightarrow B$}
		\RightLabel{$R \vee$}
		\UIC{$\Gamma \Rightarrow A \vee B$}		
	\end{prooftree}
\end{multicols}

\begin{flushleft}
	\textbf{Implication Rules:}
 \end{flushleft}
 \begin{multicols}{2}
	\begin{prooftree}
		\AXC{$\Gamma \Rightarrow A$}
		\AXC{$\Gamma, B \Rightarrow \Delta$}
		\RightLabel{$L \rightarrow$}
		\BIC{$\Gamma, \nabla (A \rightarrow B) \Rightarrow \Delta$}		
	\end{prooftree}
	\columnbreak
	\begin{prooftree}
		\AXC{$\nabla \Gamma, A \Rightarrow B$}
		\RightLabel{$R \rightarrow$}
		\UIC{$\Gamma \Rightarrow A \rightarrow B$}		
	\end{prooftree}
\end{multicols}

\begin{flushleft}
  \textbf{Modal Rule:}
\end{flushleft}
\begin{prooftree}
	\AXC{$\Gamma \Rightarrow \Delta$}
	\RightLabel{$N$}
	\UIC{$\nabla \Gamma \Rightarrow \nabla \Delta$}
\end{prooftree}


Notice that our naming scheme for the systems differs slightly with \cite{amir}. Also notice that the sequent-style systems that are introduced in the mentioned paper use sequences of formulas instead of multisets, and have an explicit exchange rule.

If we also add one or more of the following rules to the system, we will have an \emph{extension of} $\stl$, which are denoted by $\stl(S)$ where $S$ is any combination of these rules:

	\begin{prooftree}
		\RightLabel{$L$}
		\AXC{$\Gamma, A \Rightarrow \Delta$}
		\UIC{$\Gamma, \nabla A \Rightarrow \Delta$}
	\end{prooftree}

	\begin{prooftree}
		\RightLabel{$R$}
		\AXC{$\nabla \Gamma, \Sigma \Rightarrow \Delta$}
		\UIC{$\Gamma, \Sigma \Rightarrow \Delta$}
	\end{prooftree}



	\begin{prooftree}
		\RightLabel{$Fa$}
		\AXC{$\Gamma , A \Rightarrow B$}
		\UIC{$\Gamma \Rightarrow \nabla(A \rightarrow B)$}
	\end{prooftree}

	\begin{prooftree}
		\RightLabel{$Fu$}
		\AXC{$\nabla \Gamma \Rightarrow \nabla A$}
		\UIC{$\Gamma \Rightarrow A$}
	\end{prooftree}


	Now, we will introduce $\gstl$, which we then show to be equivalent with $\stl$, and also cut-free.

\begin{dfn}
	Define $\gstl$ over the language $\mathcal{L}$, to be the logic of sequent-style system defined by the same rules as $\stl$, except that the rules $Ex$, $L \wedge_1$, $L \wedge_2$, $L\vee$, $L \rightarrow$ and $N$ are replaced by the following generalized rules respectively.
\end{dfn}

\begin{prooftree}
	\AXC{}
	\RightLabel{$Ex$}
	\UIC{$\nabla^n \bot \Rightarrow$}
\end{prooftree}

\begin{multicols}{2}
	\begin{prooftree}
		\AXC{$\Gamma, \nabla^n A \Rightarrow \Delta$}
		\RightLabel{$L \wedge_1$}
		\UIC{$\Gamma, \nabla^n (A \wedge B) \Rightarrow \Delta$}
	\end{prooftree}
	\columnbreak
	\begin{prooftree}
		\AXC{$ \Gamma, \nabla^n B \Rightarrow \Delta$}
		\RightLabel{$L \wedge_2$}
		\UIC{$\Gamma, \nabla^n (A \wedge B) \Rightarrow \Delta$}		
	\end{prooftree}
\end{multicols}

\begin{prooftree}
	\AXC{$\Gamma, \nabla^n A \Rightarrow \Delta$}
	\AXC{$\Gamma, \nabla^n B \Rightarrow \Delta$}
	\RightLabel{$L \vee$}
	\BIC{$\Gamma, \nabla^n (A \vee B) \Rightarrow \Delta$}
\end{prooftree}

\begin{prooftree}
	\AXC{$\Gamma \Rightarrow \nabla^n A$}
	\AXC{$\Gamma, \nabla^n B \Rightarrow \Delta$}
	\RightLabel{$L \rightarrow$}
	\BIC{$\Gamma, \nabla^{n+1} (A \rightarrow B) \Rightarrow \Delta$}
\end{prooftree}	
Notice that all the rules above are just generalizations of their corresponding rules in $\stl$.\\

To show the equivalnce of two systems, we will use the following lemmas. Notice that the proof-trees are constructible in $\stl(S)$ for $S \subseteq \{ L, R, Fa, Fu \}$.

\begin{lem}\label{lem:l-nabla-dist-and} For all $n \geq 0$, $\stl(S) \vdash \nabla^n (A \wedge B) \Rightarrow \nabla^n A \wedge \nabla^n B$.
\end{lem}
\begin{proof}\quad
	\begin{prooftree}
		\AXC{}
		\RightLabel{$Id$}
		\UIC{$A \Rightarrow A$}
		\RightLabel{$L \wedge_1$}
		\UIC{$A \wedge B \Rightarrow A$}
		\RightLabel{$N$} \doubleLine
		\UIC{$\nabla^n (A \wedge B) \Rightarrow \nabla^n A$}

		\AXC{}
		\RightLabel{$Id$}
		\UIC{$B \Rightarrow B$}
		\RightLabel{$L \wedge_2$}
		\UIC{$A \wedge B \Rightarrow B$}
		\RightLabel{$N$} \doubleLine	
		\UIC{$\nabla^n (A \wedge B) \Rightarrow \nabla^n B$}
		
		\RightLabel{$R \wedge$}
		\BIC{$\nabla^n (A \wedge B) \Rightarrow \nabla^n A \wedge \nabla^n B$}
	\end{prooftree}
\end{proof}

\begin{lem} \label{lem:l-nabla-box} $\stl(S) \vdash \nabla (\top \rightarrow A) \Rightarrow A$.
\end{lem}
\begin{proof}\quad
	\begin{prooftree}
		\AXC{}
		\RightLabel{$Ta$}
		\UIC{$\Rightarrow \top$}
	
		\AXC{}
		\RightLabel{$Id$}
		\UIC{$A \Rightarrow A$}
	
		\RightLabel{$L \rightarrow$}
		\BIC{$\nabla (\top \rightarrow A) \Rightarrow A$}
	\end{prooftree}
\end{proof}

\begin{lem}\label{lem:l-box-nabla} $\stl(S) \vdash A \Rightarrow \top \rightarrow \nabla A$.
\end{lem}
\begin{proof}\quad
	\begin{prooftree}
		\AXC{}
		\RightLabel{$Id$}
		\UIC{$\nabla A \Rightarrow \nabla A$}
		
		\RightLabel{$Lw$}
		\UIC{$\nabla A , \top \Rightarrow \nabla A$}

		\RightLabel{$R \rightarrow$}
		\UIC{$A \Rightarrow \top \rightarrow \nabla A$}
	\end{prooftree}
\end{proof}

\begin{lem}\label{lem:l-nabla-dist-or} $\stl(S) \vdash \nabla (A \vee B) \Rightarrow \nabla A \vee \nabla B$.
\end{lem}
\begin{proof} Let $\mathcal{D}$ be a proof-tree we can construct for $\nabla (\top \rightarrow (\nabla A \vee \nabla B)) \Rightarrow \nabla A \vee \nabla B$ from Lemma \ref{lem:l-nabla-box}.

	\begin{prooftree}
		\AXC{}
		\RightLabel{$Id$}
		\UIC{$\nabla A \Rightarrow \nabla A$}
		\RightLabel{$R\vee_1$}
		\UIC{$\nabla A \Rightarrow \nabla A \vee \nabla B$}
		\RightLabel{$Lw$}
		\UIC{$\nabla A , \top \Rightarrow \nabla A \vee \nabla B$}
		\RightLabel{$R \rightarrow$}
		\UIC{$A \Rightarrow \top \rightarrow (\nabla A \vee \nabla B)$}

		\AXC{}
		\RightLabel{$Id$}
		\UIC{$\nabla B \Rightarrow \nabla B$}
		\RightLabel{$R\vee_2$}
		\UIC{$\nabla B \Rightarrow \nabla A \vee \nabla B$}
		\RightLabel{$Lw$}
		\UIC{$\nabla B , \top \Rightarrow \nabla A \vee \nabla B$}
		\RightLabel{$R \rightarrow$}
		\UIC{$B \Rightarrow \top \rightarrow (\nabla A \vee \nabla B)$}

		\RightLabel{$L\vee$}
		\BIC{$A \vee B \Rightarrow \top \rightarrow (\nabla A \vee \nabla B)$}
		\RightLabel{$N$}
		\UIC{$\nabla (A \vee B) \Rightarrow \nabla (\top \rightarrow (\nabla A \vee \nabla B))$}

		\AXC{$\mathcal{D}$}

		\RightLabel{$Cut$}
		\BIC{$\nabla (A \vee B) \Rightarrow \nabla A \vee \nabla B$}
	\end{prooftree}
\end{proof}

\begin{lem}\label{lem:l-nabla-n-dist-or} For all $n \geq 0$, $\stl(S) \vdash \nabla^n (A \vee B) \Rightarrow \nabla^n A \vee \nabla^n B$.
\end{lem}
\begin{proof} The proof is trivial when $n = 0$. Let $\mathcal{D}_1$ be the proof-tree of Lemma \ref{lem:l-nabla-dist-or}, which proves the case for $n = 1$. For any $n > 1$ we have

	\begin{prooftree}
		\AXC{$\mathcal{D}_{n-1}$}
		\noLine
		\UIC{$\nabla^{n-1} (A \vee B) \Rightarrow \nabla^{n-1} A \vee \nabla^{n-1} B$}
		\RightLabel{$N$}
		\UIC{$\nabla^n (A \vee B) \Rightarrow \nabla (\nabla^{n-1} A \vee \nabla^{n-1} B)$}

		\AXC{$\mathcal{D}_1$}
		\noLine
		\UIC{$\nabla (\nabla^{n-1} A \vee \nabla^{n-1} B) \Rightarrow \nabla^n A \vee \nabla^n B$}
		
		\RightLabel{$Cut$} \LeftLabel{$\mathcal{D}_n:$}
		\BIC{$\nabla^n (A \vee B) \Rightarrow \nabla^n A \vee \nabla^n B$}
	\end{prooftree}
\end{proof}

\begin{lem}\label{lem:l-nabla-bot} $\stl(S) \vdash \nabla \bot \Rightarrow \bot$.
\end{lem}
\begin{proof} Let $\mathcal{D}$ be a proof-tree for $\nabla (\top \rightarrow \bot) \Rightarrow \bot$ which we have by Lemma \ref{lem:l-nabla-box}.
	\begin{prooftree}
		\AXC{}
		\RightLabel{$Ex$}
		\UIC{$\bot \Rightarrow$}
		\RightLabel{$Rw$}
		\UIC{$\bot \Rightarrow \top \rightarrow \bot$}
		\RightLabel{$N$}
		\UIC{$\nabla \bot \Rightarrow \nabla (\top \rightarrow \bot)$}

		\AXC{$\mathcal{D}$}

		\RightLabel{$Cut$}
		\BIC{$\nabla \bot \Rightarrow \bot$}
	\end{prooftree}	
\end{proof}

\begin{lem}\label{lem:l-nabla-n-bot} For $n > 0$, $\stl(S) \vdash \nabla^n \bot \Rightarrow \bot$.
\end{lem}
\begin{proof} We will prove a stronger version: For $n \geq m > 0$, $\stl(S) \vdash \nabla^n \bot \Rightarrow \nabla^{n-m} \bot$. Let $\mathcal{D}_1$ be the proof-tree of Lemma \ref{lem:l-nabla-bot} which handles $n = m = 1$. Using induction on $m$, and denoting the proof-tree for $\nabla^n \bot \Rightarrow \nabla^{n-(m-1)} \bot$ from the induction hypothesis by IH, we have for $n > 1$
	\begin{prooftree}
		\AXC{IH}
		\noLine
		\UIC{$\nabla^n \bot \Rightarrow \nabla^{n-(m-1)} \bot$}

		\AXC{$\mathcal{D}_1$}
		\noLine
		\UIC{$\nabla \bot \Rightarrow \bot$}
		\doubleLine \RightLabel{$N^{(n-m)}$}
		\UIC{$\nabla^{n-(m-1)} \bot \Rightarrow \nabla^{n-m} \bot$}

		\RightLabel{$Cut$}
		\BIC{$\nabla^n \bot \Rightarrow \nabla^{n-m} \bot$}
	\end{prooftree}
\end{proof}

\begin{lem}\label{lem:l-nabla-dist-si} For any $n \geq 0$, $\stl(S) \vdash \nabla^n (A \rightarrow B) \Rightarrow \nabla^n A \rightarrow \nabla^n B$.
\end{lem}
\begin{proof}\quad
	\begin{prooftree}
		\AXC{}
		\RightLabel{$Id$}
		\UIC{$A \Rightarrow A$}
		
		\AXC{}
		\RightLabel{$Id$}
		\UIC{$B \Rightarrow B$}
		\RightLabel{$Lw$}
		\UIC{$A , B \Rightarrow B$}
		
		\RightLabel{$L \rightarrow$}
		\BIC{$\nabla (A \rightarrow B) , A \Rightarrow B$}
		\RightLabel{$N^{(n)}$} \doubleLine
		\UIC{$\nabla^{n+1} (A \rightarrow B) , \nabla^n A \Rightarrow \nabla^n B$}
		\RightLabel{$R \rightarrow$}
		\UIC{$\nabla^n (A \rightarrow B) \Rightarrow \nabla^n A \rightarrow \nabla^n B$}
	\end{prooftree}
\end{proof}


In the rest of this paper, by the \emph{height of a proof-tree} $\mathcal{D}$, denoted by $h(\mathcal{D})$, we mean the number of rule instances in its longest branch.

The theorem below shows that $\stl$ (and its extensions) deduce exactly the same sequents as $\gstl$ (and its extensions).

\begin{thm}\label{thm:stl-eq-gstl}
	Let $S \subseteq \{L, R, Fa, Fu\}$. For any sequent $\Gamma \Rightarrow \Delta$ in the language $\mathcal{L}$, $\stl(S) \vdash \Gamma \Rightarrow \Delta$ iff $\gstl(S) \vdash \Gamma \Rightarrow \Delta$.
\end{thm}
\begin{proof}
	One direction easily follows from the fact that all rules of $\stl(S)$ are just instances of $\gstl(S)$'s rules.
	For the other direction, we will use case analysis for the last rule in the proof-tree of $\Gamma \Rightarrow \Delta$ in $\gstl(S)$, which we call $\mathcal{D}$, and construct a proof-tree for it in $\stl(S)$ in each case.
	
	First, observe that $Id$ and $Ta$ are present in $\stl(S)$ and Lemma \ref{lem:l-nabla-n-bot} handles the $Ex$ case.
	For the other rules, use induction on the length of $\mathcal{D}$; the induction hypothesis will provide a proof-tree in $\stl(S)$ for the subtree(s) of $\mathcal{D}$.
	For the rules that are common between two systems, just apply the same rule (in $\stl(S)$) on the proof-tree(s) from the induction hypothesis to reach the desired sequent. For example, if $\mathcal{D}$ ends with $R \vee$, it suffices to apply $R \vee$ (of $\stl(S)$) on the proof-tree that we get from the induction hypothesis.
	In the cases for $\gstl(S)$'s stronger rules, which are $L \wedge_1$, $L \wedge_2$, $L \vee$ and $L \rightarrow$, do the same, and also cut the sequents proved in Lemmas \ref{lem:l-nabla-dist-and}, \ref{lem:l-nabla-dist-or} or \ref{lem:l-nabla-dist-si} into the resulting sequent.
	The case for $N$ divides into two further cases. One case is when $\Delta = A$ for some formula $A$, which is again handled by applying $N$ on the sequent from the induction hypothesis.
	The other case is when $\Delta = \{\}$, so we have $\Gamma \Rightarrow$ from the induction hypothesis, on the right of which we first introduce $\bot$ using $Rw$, and then apply $N$.
	Then we can cut it into the sequent proved in Lemma \ref{lem:l-nabla-bot}, and then into $Ex$, to derive $\nabla \Gamma \Rightarrow$ as was desired.
\end{proof}

[introducing iSTL, the conservative extension with intuitionistic implication]

[introducing the equivalent cut-free system, iGSTL]

[diagram]

\section{Cut-elimination theorem}
[cut reduction]

[cut elimination]

\subsection{applications}
[visser rule]

[disjuction property]

[subformula property]

\section{Interpolation theorems}
[deductive interpolation for iSTL+L]

[craig's interpolation for intuitionistic extension]

\section{Conclusion and future works}

\section{Acknowledgement}

\bibliographystyle{abbrv}
\bibliography{refs}
\end{document}
